Numerous changes to proof scripts were required by the change in restricted quantification.
A few statements changed too. This was necessary because if you
write
  !w :: PWORDLEN n. M w n
then you must consistently treat PWORDLEN as a set, so
  PWORDLEN n w
elsewhere must be changed to
  w IN PWORDLEN n

(Of course, you can always move between these forms with
SPECIFICATION, but that's not a nice solution in terms of
keeping the proof scripts short.)

src/word/src/wordLib.sig
@@ -3,6 +3,7 @@
 (* DESCRIPTION   : Signature for word conversions and tactics           *)
 (* AUTHOR	 : P Curzon 					        *)
 (* DATE		 : June 1993						*)
+(* UPDATED       : Joe Hurd, November 2001, for new res_quan library    *)
 (*                                                                      *)
 (* =====================================================================*)
 
