src/word/theories/word_bitopScript.sml
@@ -1,10 +1,11 @@
 (* =====================================================================*)
-(* FILE: mk_word_bitop.ml	    DATE: 14 Aug 1992			*)
-(* AUTHOR: Wai WONG  	    	    					*)
-(* TRANSLATOR: Paul Curzon  1 June 1993, September 1994			*)
-(* Writes: word_bitop.th	    	    				*)
-(* Uses: Libraries: arith res_quan					*)
-(* Description: Creates a theore for generic word bitwise operations	*)
+(* FILE: mk_word_bitop.ml           DATE: 14 Aug 1992                   *)
+(* AUTHOR: Wai WONG                                                     *)
+(* TRANSLATOR: Paul Curzon  1 June 1993, September 1994                 *)
+(* UPDATED for new res_quan theories by Joe Hurd, November 2001         *)
+(* Writes: word_bitop.th                                                *)
+(* Uses: Libraries: arith res_quan                                      *)
+(* Description: Creates a theore for generic word bitwise operations    *)
 (* =====================================================================*)
 (* PC 18/11/93: SEG ->WSEG *)
 
@@ -12,7 +13,8 @@
 open HolKernel Parse boolLib Prim_rec;
 open Base numLib res_quanLib;
 open rich_listTheory pairTheory arithmeticTheory prim_recTheory numTheory;
-open Cond_rewrite Res_quan word_baseTheory;
+open Cond_rewrite word_baseTheory;
+open res_quanTheory bossLib pred_setTheory;
 
 infix THEN THENL THENC ORELSE ORELSEC;
 
@@ -34,59 +36,69 @@ val word_INDUCT_TAC =
     end;
 
 val RESQ_WORDLEN_TAC =
-    (CONV_TAC RESQ_FORALL_CONV THEN word_INDUCT_TAC
-     THEN PURE_ONCE_REWRITE_TAC[word_baseTheory.PWORDLEN_DEF]
+    (CONV_TAC RES_FORALL_CONV THEN word_INDUCT_TAC
+     THEN PURE_ONCE_REWRITE_TAC[word_baseTheory.IN_PWORDLEN]
      THEN GEN_TAC THEN DISCH_TAC);
 
-
+val GGEN_TAC = RESQ_GEN_TAC ORELSE GEN_TAC;
 
 (* --------------------------------------------------------------------- *)
-(* We begin with some lemmas about lists. They are used in the proofs.	*)
+(* We begin with some lemmas about lists. They are used in the proofs.  *)
 (* --------------------------------------------------------------------- *)
 val LASTN_BUTLASTN_SEG = prove(
     (--`!m k (l:'a list). (m + k) <= (LENGTH l) ==>
      (LASTN m (BUTLASTN k l) = SEG m((LENGTH l) - (m + k))l)`--),
     let val lem1 = ARITH_PROVE
-    	 (--`!l m k. (m+k)<=l ==>((m + (l - (m + k))) = (l - k))`--)
+         (--`!l m k. (m+k)<=l ==>((m + (l - (m + k))) = (l - k))`--)
     val lem2 = ARITH_PROVE
-    	 (--`!l m k. (m+k)<=l ==> ((l - (m + (l - (m + k)))) = k)`--)
+         (--`!l m k. (m+k)<=l ==> ((l - (m + (l - (m + k)))) = k)`--)
     in
     REPEAT STRIP_TAC THEN COND_REWRITE1_TAC SEG_LASTN_BUTLASTN THENL[
         IMP_RES_THEN (fn t => REWRITE_TAC[t])lem1
-    	THEN MATCH_ACCEPT_TAC SUB_LESS_EQ,
+        THEN MATCH_ACCEPT_TAC SUB_LESS_EQ,
         IMP_RES_THEN (fn t => REWRITE_TAC[t])lem2]
     end);
 
 (*---------------------------------------------------------------*)
-(* Bitwise operators 	    	    				 *)
+(* Bitwise operators                                             *)
 (*---------------------------------------------------------------*)
 
 (*---------------------------------------------------------------*)
-(* PBITOP (op:'a word -> 'b word) is true if op is a bitwise	 *)
-(* unary operator    	    	    				 *)
+(* PBITOP (op:'a word -> 'b word) is true if op is a bitwise     *)
+(* unary operator                                                *)
 (*---------------------------------------------------------------*)
 
-val PBITOP_DEF = new_definition("PBITOP_DEF",
-    (--`PBITOP (op:'a word -> 'b word) =
-     !n. !w:'a word ::PWORDLEN n. PWORDLEN n (op w) /\
-     !m k. ((m + k) <= n) ==> (op(WSEG m k w) = WSEG m k (op w))`--));
+val PBITOP_def = Define
+  `PBITOP =
+   {(op:'a word -> 'b word) |
+    !n. !w:'a word ::PWORDLEN n. (op w) IN PWORDLEN n /\
+    !m k. ((m + k) <= n) ==> (op(WSEG m k w) = WSEG m k (op w))}`;
+
+val IN_PBITOP = store_thm
+  ("IN_PBITOP",
+   ``!op.
+       op IN PBITOP =
+       !n. !w:'a word ::PWORDLEN n. (op w) IN PWORDLEN n /\
+       !m k. ((m + k) <= n) ==> (op(WSEG m k w) = WSEG m k (op w))``,
+   RW_TAC std_ss [PBITOP_def, GSPECIFICATION]);
 
 val PBITOP_PWORDLEN = store_thm("PBITOP_PWORDLEN",
     (--`!op:('a)word->('b)word::PBITOP. !n. !w:('a)word::PWORDLEN n.
-     (PWORDLEN n (op w))`--),
-    REPEAT GGEN_TAC THEN IMP_RES_TAC PBITOP_DEF THEN RESQ_RES_TAC);
+     ((op w) IN PWORDLEN n)`--),
+    REPEAT (RESQ_GEN_TAC ORELSE GEN_TAC)
+    THEN IMP_RES_TAC IN_PBITOP THEN RESQ_RES_TAC);
 
 val PBITOP_WSEG = store_thm("PBITOP_WSEG",
     (--`!op:('a)word->('b)word::PBITOP. !n. !w:('a)word::PWORDLEN n.
      !m k. ((m + k) <= n) ==> (op(WSEG m k w) = WSEG m k (op w))`--),
     RESQ_GEN_TAC THEN GEN_TAC THEN RESQ_GEN_TAC
-    THEN IMP_RES_TAC PBITOP_DEF THEN RESQ_RES_TAC);
+    THEN IMP_RES_TAC IN_PBITOP THEN RESQ_RES_TAC);
 
 val PBITOP_BIT = store_thm("PBITOP_BIT",
     (--`!op:('a)word->('b)word::PBITOP.
      !n. !w:'a word ::PWORDLEN n. !k. (k < n) ==>
      (op(WORD[BIT k w]) = WORD[BIT k (op w)])`--),
-    RESQ_HALF_GEN_TAC THEN GEN_TAC THEN PURE_ONCE_REWRITE_TAC[PBITOP_DEF]
+    CONV_TAC RES_FORALL_CONV THEN GEN_TAC THEN PURE_ONCE_REWRITE_TAC[IN_PBITOP]
     THEN DISCH_TAC THEN GEN_TAC THEN RESQ_GEN_TAC
     THEN REPEAT STRIP_TAC THEN RESQ_RES_TAC
     THEN RESQ_IMP_RES_TAC (CONV_RULE (ONCE_DEPTH_CONV SYM_CONV) WSEG_BIT)
@@ -98,27 +110,41 @@ val BIT_op_EXISTS = prove(
     (--`!op:('a)word->('b)word::PBITOP. ?op':'a->'b. !n. !w:('a)word::PWORDLEN n.
      !k. (k < n) ==> ((BIT k (op w)) = (op'(BIT k w)))`--),
     RESQ_GEN_TAC THEN EXISTS_TAC(--`\b:'a.BIT 0((op:('a)word->('b)word)(WORD[b]))`--)
-    THEN GEN_TAC THEN RESQ_HALF_GEN_TAC THEN GEN_TAC THEN REPEAT STRIP_TAC
+    THEN GEN_TAC THEN CONV_TAC RES_FORALL_CONV THEN GEN_TAC
+    THEN REPEAT STRIP_TAC
+    THEN RW_TAC std_ss []
     THEN RESQ_IMP_RES_TAC PBITOP_BIT THEN RES_THEN SUBST1_TAC
     THEN REWRITE_TAC[BIT0]);
 
 (*---------------------------------------------------------------*)
 (* PBITBOP (op:'a word -> 'b word -> 'c word) is true if op is a *)
-(*  bitwise binary operator  	    				*)
+(*  bitwise binary operator                                     *)
 (*---------------------------------------------------------------*)
 
-val PBITBOP_DEF = new_definition("PBITBOP_DEF",
-    (--`PBITBOP (op:'a word  -> 'b word -> 'c word) =
-     !n. !w1:'a word ::PWORDLEN n. !w2:'b word ::PWORDLEN n.
-     (PWORDLEN n (op w1 w2)) /\
-     !m k. ((m + k) <= n) ==>
-     (op (WSEG m k w1) (WSEG m k w2) = WSEG m k (op w1 w2))`--));
+val PBITBOP_def = Define
+  `PBITBOP =
+   {(op:'a word  -> 'b word -> 'c word) |
+    !n. !w1:'a word ::PWORDLEN n. !w2:'b word ::PWORDLEN n.
+    ((op w1 w2) IN PWORDLEN n) /\
+    !m k. ((m + k) <= n) ==>
+    (op (WSEG m k w1) (WSEG m k w2) = WSEG m k (op w1 w2))}`;
+
+val IN_PBITBOP = store_thm
+  ("IN_PBITBOP",
+   ``!op.
+       op IN PBITBOP =
+       !n. !w1:'a word ::PWORDLEN n. !w2:'b word ::PWORDLEN n.
+       ((op w1 w2) IN PWORDLEN n) /\
+       !m k. ((m + k) <= n) ==>
+       (op (WSEG m k w1) (WSEG m k w2) = WSEG m k (op w1 w2))``,
+   RW_TAC std_ss [PBITBOP_def, GSPECIFICATION]);
 
 val PBITBOP_PWORDLEN = store_thm("PBITBOP_PWORDLEN",
     (--`!op:'a word  -> 'b word -> 'c word::PBITBOP.
      !n. !w1:'a word ::PWORDLEN n. !w2:'b word ::PWORDLEN n.
-     (PWORDLEN n (op w1 w2))`--),
-    REPEAT GGEN_TAC THEN IMP_RES_TAC PBITBOP_DEF THEN RESQ_RES_TAC);
+     ((op w1 w2) IN PWORDLEN n)`--),
+    REPEAT (RESQ_GEN_TAC ORELSE GEN_TAC)
+    THEN IMP_RES_TAC IN_PBITBOP THEN RESQ_RES_TAC);
 
 val PBITBOP_WSEG = store_thm("PBITBOP_WSEG",
     (--`!op:'a word  -> 'b word -> 'c word::PBITBOP.
@@ -126,7 +152,7 @@ val PBITBOP_WSEG = store_thm("PBITBOP_WSEG",
      !m k. ((m + k) <= n) ==>
      (op (WSEG m k w1) (WSEG m k w2) = WSEG m k (op w1 w2))`--),
     RESQ_GEN_TAC THEN GEN_TAC THEN  REPEAT RESQ_GEN_TAC
-    THEN IMP_RES_TAC PBITBOP_DEF
+    THEN IMP_RES_TAC IN_PBITBOP
     THEN RESQ_RES_TAC
     THEN ASM_REWRITE_TAC[]);
 
@@ -145,8 +171,8 @@ val PBITBOP_EXISTS = store_thm("PBITBOP_EXISTS",
     end);
 
 (*---------------------------------------------------------------*)
-(* WMAP: applies a function to every bit of a word		*)
-(* WMAP: ('a->'b) -> 'a word -> 'b word				*)
+(* WMAP: applies a function to every bit of a word              *)
+(* WMAP: ('a->'b) -> 'a word -> 'b word                         *)
 (*---------------------------------------------------------------*)
 
 val WMAP_DEF = new_recursive_definition {
@@ -159,9 +185,9 @@ val WMAP_DEF = new_recursive_definition {
  };
 
 val WMAP_PWORDLEN = store_thm("WMAP_PWORDLEN",
-    (--`!w::PWORDLEN n. !f:'a->'b. PWORDLEN n (WMAP f w)`--),
-    RESQ_HALF_GEN_TAC THEN word_INDUCT_TAC
-    THEN REWRITE_TAC[WMAP_DEF,PWORDLEN_DEF,LENGTH_MAP]);
+    (--`!w::PWORDLEN n. !f:'a->'b. (WMAP f w) IN PWORDLEN n`--),
+    CONV_TAC RES_FORALL_CONV THEN word_INDUCT_TAC
+    THEN REWRITE_TAC[WMAP_DEF,IN_PWORDLEN,LENGTH_MAP]);
 
 val WMAP0 = store_thm("WMAP_0",
     (--`!f:'a->'b. (WMAP f (WORD[]:'a word) = (WORD []:'b word))`--),
@@ -172,16 +198,16 @@ val WMAP_BIT = store_thm("WMAP_BIT",
      !f:'a->'b. BIT k (WMAP f w) = f (BIT k w)`--),
     GEN_TAC THEN RESQ_WORDLEN_TAC THEN REPEAT STRIP_TAC
     THEN REWRITE_TAC[BIT_DEF,WMAP_DEF]
-    THEN MATCH_MP_TAC ELL_MAP THEN FIRST_ASSUM (SUBST1_TAC o SYM)
+    THEN MATCH_MP_TAC ELL_MAP THEN FIRST_ASSUM (SUBST1_TAC)
     THEN FIRST_ASSUM ACCEPT_TAC);
 
 val WMAP_WSEG = store_thm("WMAP_WSEG",
     (--`!n. !w :: PWORDLEN n.
      !m k. (m + k) <= n ==>
      !f:'a->'b. (WMAP f(WSEG m k w) = WSEG m k(WMAP f w))`--),
-    GEN_TAC THEN RESQ_HALF_GEN_TAC THEN word_INDUCT_TAC
-    THEN REWRITE_TAC[WMAP_DEF,WSEG_DEF,PWORDLEN_DEF,WORD_11]
-    THEN GEN_TAC THEN DISCH_THEN SUBST1_TAC
+    GEN_TAC THEN CONV_TAC RES_FORALL_CONV THEN word_INDUCT_TAC
+    THEN REWRITE_TAC[WMAP_DEF,WSEG_DEF,IN_PWORDLEN,WORD_11]
+    THEN GEN_TAC THEN DISCH_THEN (SUBST1_TAC o SYM)
     THEN REPEAT STRIP_TAC THEN COND_REWRITE1_TAC BUTLASTN_MAP THENL[
      IMP_RES_TAC LESS_EQ_SPLIT,
      COND_REWRITE1_TAC LASTN_MAP THENL[
@@ -191,13 +217,12 @@ val WMAP_WSEG = store_thm("WMAP_WSEG",
       REFL_TAC]]);
 
 val WMAP_PBITOP = store_thm("WMAP_PBITOP",
-    (--`!f:'a->'b. PBITOP (WMAP f)`--),
-    GEN_TAC THEN PURE_ONCE_REWRITE_TAC[PBITOP_DEF]
+    (--`!f:'a->'b. (WMAP f) IN PBITOP`--),
+    GEN_TAC THEN PURE_ONCE_REWRITE_TAC[IN_PBITOP]
     THEN GEN_TAC THEN RESQ_GEN_TAC THEN CONJ_TAC THENL[
      RESQ_IMP_RES_THEN MATCH_ACCEPT_TAC WMAP_PWORDLEN,
      REPEAT STRIP_TAC THEN RESQ_IMP_RES_TAC WMAP_WSEG
      THEN RES_THEN MATCH_ACCEPT_TAC]);
-
 
 val WMAP_WCAT = store_thm("WMAP_WCAT",
     (--`!w1 w2 (f:'a->'b).
@@ -211,7 +236,7 @@ val WMAP_o = store_thm("WMAP_o",
     THEN REWRITE_TAC[WMAP_DEF,MAP_MAP_o]);
 
 (*---------------------------------------------------------------*)
-(* FORALLBITS : ('a -> bool) -> ('a)word -> bool			*)
+(* FORALLBITS : ('a -> bool) -> ('a)word -> bool                        *)
 (*---------------------------------------------------------------*)
 
 val FORALLBITS_DEF = new_recursive_definition {
@@ -226,28 +251,29 @@ val FORALLBITS_DEF = new_recursive_definition {
 val FORALLBITS = store_thm("FORALLBITS",
     (--`!n. !w:('a)word::PWORDLEN n. !P.
      FORALLBITS P w = (!k. k < n ==> P(BIT k w))`--),
-    GEN_TAC THEN RESQ_HALF_GEN_TAC THEN word_INDUCT_TAC THEN GEN_TAC
-    THEN PURE_ONCE_REWRITE_TAC[PWORDLEN_DEF,FORALLBITS_DEF,BIT_DEF]
+    GEN_TAC THEN CONV_TAC RES_FORALL_CONV THEN word_INDUCT_TAC THEN GEN_TAC
+    THEN PURE_ONCE_REWRITE_TAC[IN_PWORDLEN,FORALLBITS_DEF,BIT_DEF]
     THEN MAP_EVERY SPEC_TAC [((--`n:num`--),(--`n:num`--)),
                              ((--`l:'a list`--),(--`l:'a list`--))]
     THEN LIST_INDUCT_TAC THEN REPEAT GEN_TAC
     THEN PURE_ONCE_REWRITE_TAC[LENGTH,ALL_EL]
-    THEN DISCH_THEN SUBST1_TAC THENL[
+    THEN DISCH_THEN (SUBST1_TAC o SYM) THENL[
       REWRITE_TAC[NOT_LESS_0],
       GEN_TAC THEN EQ_TAC THEN PURE_ONCE_REWRITE_TAC[LESS_THM] THENL[
-    	STRIP_TAC THEN GEN_TAC
-    	THEN DISCH_THEN (DISJ_CASES_THEN2 SUBST1_TAC ASSUME_TAC) THENL[
-    	  ASM_REWRITE_TAC[ELL_LENGTH_CONS],
-    	  IMP_RES_THEN (fn t => REWRITE_TAC[t]) ELL_CONS
-    	  THEN FIRST_ASSUM (SUBST_ALL_TAC o SPEC_ALL o (REWRITE_RULE[]) o
-    	    (SPEC(--`LENGTH (l:'a list)`--))) THEN RES_TAC],
+        STRIP_TAC THEN GEN_TAC
+        THEN DISCH_THEN (DISJ_CASES_THEN2 SUBST1_TAC ASSUME_TAC) THENL[
+          ASM_REWRITE_TAC[ELL_LENGTH_CONS],
+          IMP_RES_THEN (fn t => REWRITE_TAC[t]) ELL_CONS
+          THEN FIRST_ASSUM (SUBST_ALL_TAC o SPEC_ALL o (REWRITE_RULE[]) o
+            (SPEC(--`LENGTH (l:'a list)`--))) THEN RES_TAC],
       DISCH_TAC THEN CONJ_TAC THEN POP_ASSUM MP_TAC
+      THEN (PURE_ONCE_REWRITE_TAC [EQ_SYM_EQ])
       THEN FIRST_ASSUM (SUBST_ALL_TAC o SPEC_ALL o (REWRITE_RULE[]) o
-    	    (SPEC(--`LENGTH (l:'a list)`--))) THENL[
+            (SPEC(--`LENGTH (l:'a list)`--))) THENL[
         CONV_TAC LEFT_IMP_FORALL_CONV
         THEN EXISTS_TAC(--`LENGTH (l:'a list)`--)
         THEN REWRITE_TAC[LESS_REFL,ELL_LENGTH_CONS],
-    	REPEAT STRIP_TAC THEN RES_THEN MP_TAC
+        REPEAT STRIP_TAC THEN RES_THEN MP_TAC
         THEN IMP_RES_THEN (fn t => REWRITE_TAC[t]) ELL_CONS]]]);
 
 
@@ -255,14 +281,14 @@ val FORALLBITS_WSEG = store_thm("FORALLBITS_WSEG",
     (--`!n. !w:('a)word::PWORDLEN n. !P.
      FORALLBITS P w ==>
      !m k. (m + k) <= n ==> FORALLBITS P (WSEG m k w)`--),
-    GEN_TAC THEN RESQ_HALF_GEN_TAC THEN word_INDUCT_TAC
-    THEN REWRITE_TAC[WSEG_DEF,PWORDLEN_DEF,FORALLBITS_DEF]
-    THEN GEN_TAC THEN DISCH_THEN SUBST1_TAC
+    GEN_TAC THEN CONV_TAC RES_FORALL_CONV THEN word_INDUCT_TAC
+    THEN REWRITE_TAC[WSEG_DEF,IN_PWORDLEN,FORALLBITS_DEF]
+    THEN GEN_TAC THEN DISCH_THEN (SUBST1_TAC o SYM)
     THEN SPEC_TAC((--`l:'a list`--),(--`l:'a list`--))
     THEN SNOC_INDUCT_TAC THENL[
      REWRITE_TAC[LENGTH,ALL_EL] THEN REPEAT STRIP_TAC
      THEN IMP_RES_THEN  (SUBST_TAC o CONJUNCTS o
-    	 (PURE_ONCE_REWRITE_RULE[ADD_EQ_0])) LESS_EQ_0_EQ
+         (PURE_ONCE_REWRITE_RULE[ADD_EQ_0])) LESS_EQ_0_EQ
      THEN REWRITE_TAC[LASTN,BUTLASTN,ALL_EL],
      REWRITE_TAC[LENGTH_SNOC,ALL_EL_SNOC]
      THEN REPEAT GEN_TAC THEN STRIP_TAC THEN INDUCT_TAC THENL[
@@ -282,7 +308,7 @@ val FORALLBITS_WCAT = store_thm("FORALLBITS_WCAT",
     THEN REWRITE_TAC[FORALLBITS_DEF,WCAT_DEF,ALL_EL_APPEND]);
 
 (*---------------------------------------------------------------*)
-(* EXISTSABIT : ('a -> bool) -> ('a)word -> bool		 *)
+(* EXISTSABIT : ('a -> bool) -> ('a)word -> bool                 *)
 (*---------------------------------------------------------------*)
 
 val EXISTSABIT_DEF = new_recursive_definition
@@ -309,9 +335,9 @@ val NOT_FORALLBITS = store_thm("NOT_FORALLBITS",
 val EXISTSABIT_BIT = store_thm("EXISTSABIT",
     (--`!n. !w:('a)word::PWORDLEN n. !P.
      EXISTSABIT P w = ?k. k < n /\ P(BIT k w)`--),
-    GEN_TAC THEN RESQ_HALF_GEN_TAC THEN word_INDUCT_TAC THEN GEN_TAC
-    THEN PURE_ONCE_REWRITE_TAC[PWORDLEN_DEF,EXISTSABIT_DEF,BIT_DEF]
-    THEN DISCH_THEN SUBST1_TAC
+    GEN_TAC THEN CONV_TAC RES_FORALL_CONV THEN word_INDUCT_TAC THEN GEN_TAC
+    THEN PURE_ONCE_REWRITE_TAC[IN_PWORDLEN,EXISTSABIT_DEF,BIT_DEF]
+    THEN DISCH_THEN (SUBST1_TAC o SYM)
     THEN MAP_EVERY SPEC_TAC
          [((--`n:num`--),(--`n:num`--)),((--`l:'a list`--),(--`l:'a list`--))]
     THEN LIST_INDUCT_TAC THEN REPEAT GEN_TAC
@@ -320,31 +346,31 @@ val EXISTSABIT_BIT = store_thm("EXISTSABIT",
        STRIP_TAC THENL[
       EXISTS_TAC (--`LENGTH(l:'a list)`--)
       THEN ASM_REWRITE_TAC[ELL_LENGTH_CONS],
-    	RES_TAC THEN EXISTS_TAC (--`k:num`--)
+        RES_TAC THEN EXISTS_TAC (--`k:num`--)
         THEN COND_REWRITE1_TAC ELL_CONS THEN ASM_REWRITE_TAC[]],
       PURE_ONCE_REWRITE_TAC[RIGHT_AND_OVER_OR]
       THEN DISCH_THEN (STRIP_THM_THEN
-    	(DISJ_CASES_THEN2 STRIP_ASSUME_TAC MP_TAC)) THENL[
-    	FIRST_ASSUM SUBST_ALL_TAC
+        (DISJ_CASES_THEN2 STRIP_ASSUME_TAC MP_TAC)) THENL[
+        FIRST_ASSUM SUBST_ALL_TAC
         THEN RULE_ASSUM_TAC (REWRITE_RULE[ELL_LENGTH_CONS])
-    	THEN DISJ1_TAC THEN FIRST_ASSUM ACCEPT_TAC,
-    	DISCH_THEN (CONJUNCTS_THEN2 ASSUME_TAC MP_TAC)
-    	THEN COND_REWRITE1_TAC ELL_CONS THEN DISCH_TAC THEN RES_TAC
-    	THEN DISJ2_TAC THEN FIRST_ASSUM ACCEPT_TAC]]);
+        THEN DISJ1_TAC THEN FIRST_ASSUM ACCEPT_TAC,
+        DISCH_THEN (CONJUNCTS_THEN2 ASSUME_TAC MP_TAC)
+        THEN COND_REWRITE1_TAC ELL_CONS THEN DISCH_TAC THEN RES_TAC
+        THEN DISJ2_TAC THEN FIRST_ASSUM ACCEPT_TAC]]);
 
 val EXISTSABIT_WSEG = store_thm("EXISTSABIT_WSEG",
     (--`!n. !w:('a)word::PWORDLEN n. !m k. ((m + k) <= n) ==>
      !P. (EXISTSABIT P (WSEG m k w)) ==> (EXISTSABIT P w)`--),
   let val lem1 = ARITH_PROVE
-     	 (--`!l m k. (m+k)<=l ==>((m + (l - (m + k))) = (l - k))`--)
+         (--`!l m k. (m+k)<=l ==>((m + (l - (m + k))) = (l - k))`--)
   in
-     GEN_TAC THEN RESQ_HALF_GEN_TAC  THEN word_INDUCT_TAC
-     THEN REWRITE_TAC[EXISTSABIT_DEF,PWORDLEN_DEF,WSEG_DEF]
-     THEN GEN_TAC THEN DISCH_THEN SUBST1_TAC
+     GEN_TAC THEN CONV_TAC RES_FORALL_CONV THEN word_INDUCT_TAC
+     THEN REWRITE_TAC[EXISTSABIT_DEF,IN_PWORDLEN,WSEG_DEF]
+     THEN GEN_TAC THEN DISCH_THEN (SUBST1_TAC o SYM)
      THEN REPEAT GEN_TAC THEN DISCH_TAC THEN GEN_TAC
      THEN COND_REWRITE1_TAC LASTN_BUTLASTN_SEG
      THEN MATCH_MP_TAC (SPECL
-     	[(--`m:num`--),(--`(LENGTH (l:'a list)) - (m + k)`--),
+        [(--`m:num`--),(--`(LENGTH (l:'a list)) - (m + k)`--),
          (--`l:'a list`--)] SOME_EL_SEG)
      THEN IMP_RES_THEN SUBST1_TAC lem1
      THEN MATCH_ACCEPT_TAC SUB_LESS_EQ
@@ -355,8 +381,9 @@ val EXISTSABIT_WCAT = store_thm("EXISTSABIT_WCAT",
      EXISTSABIT P (WCAT(w1,w2)) = (EXISTSABIT P w1 \/ EXISTSABIT P w2)`--),
     REPEAT (word_INDUCT_TAC THEN GEN_TAC) THEN GEN_TAC
     THEN REWRITE_TAC[EXISTSABIT_DEF,WCAT_DEF,SOME_EL_APPEND]);
+
 (*---------------------------------------------------------------*)
-(* Shift and rotation   	    					*)
+(* Shift and rotation                                                   *)
 (*---------------------------------------------------------------*)
 
 val SHR_DEF = new_definition("SHR_DEF",
@@ -395,14 +422,17 @@ val SHR_WSEG = store_thm("SHR_WSEG",
      !b m k. (m + k) <= n ==> 0 < m ==>
       (SHR F b(WSEG m k w) = WCAT(WORD[b],WSEG(m - 1)(k + 1)w),BIT k w) *)
 val SHR_WSEG_1F = save_thm("SHR_WSEG_1F",
-    let val th1 = SPEC_ALL(RESQ_SPEC_ALL(SPEC_ALL SHR_WSEG))
+    let val th1 = RESQ_SPECL [``n : num``, ``w : 'a word``, ``m : num``, ``k : num``] SHR_WSEG
     val {Rator = P,Rand = v} = dest_comb(hd(hyp th1))
     val ante = fst(strip_imp(concl th1))
-    val th2 = CONV_RULE(ONCE_DEPTH_CONV COND_CONV)
-    	(SPEC (--`F`--) (UNDISCH_ALL th1))
+    val th2 = SPEC ``b : 'a`` (CONV_RULE(ONCE_DEPTH_CONV COND_CONV)
+        (SPEC (--`F`--) (UNDISCH_ALL th1)))
     in
-    GEN_ALL(RESQ_GEN (v,P) (GENL[(--`m:num`--),(--`k:num`--)]
-                                (itlist DISCH ante th2)))
+    GEN_ALL
+    (CONV_RULE (HO_REWR_CONV (GSYM RES_FORALL))
+     (GEN ``w : 'a word``
+      (DISCH_ALL (GENL[``b : 'a``, ``m:num``, ``k:num``]
+                  (itlist DISCH ante th2)))))
     end);
 
 val SHR_WSEG_NF_lem1 =  ARITH_PROVE (--`0<m ==>((m-1)+1 = m)`--);
@@ -431,7 +461,7 @@ val SHR_WSEG_NF = store_thm("SHR_WSEG_NF",
                    simpLib.ASM_SIMP_TAC bossLib.arith_ss []
         THEN POP_ASSUM MP_TAC THEN MP_TAC (Q.ASSUME`0<m`)
         THEN simpLib.SIMP_TAC bossLib.arith_ss [],
-    	REFL_TAC]]);
+        REFL_TAC]]);
 
 val SHL_WSEG = store_thm("SHL_WSEG",
     (--`!n. !w:('a)word::PWORDLEN n. ! m k. ((m + k) <= n) ==> (0 < m) ==>
@@ -440,7 +470,7 @@ val SHL_WSEG = store_thm("SHL_WSEG",
             (WCAT((WSEG (m-1) k w),(WORD[b]))))))`--),
     let fun f t1 tms =
         ((IMP_RES_THEN SUBST1_TAC) o (fn th => MATCH_MP th t1)
-    	  o (PURE_ONCE_REWRITE_RULE[ADD_CLAUSES]) o (SPECL tms))
+          o (PURE_ONCE_REWRITE_RULE[ADD_CLAUSES]) o (SPECL tms))
     in
     REPEAT GGEN_TAC THEN PURE_REWRITE_TAC[SHL_DEF] THEN REPEAT DISCH_TAC
     THEN REPEAT GEN_TAC THEN PURE_ONCE_REWRITE_TAC[PAIR_EQ]
@@ -448,9 +478,9 @@ val SHL_WSEG = store_thm("SHL_WSEG",
       RESQ_IMP_RES_THEN (IMP_RES_THEN SUBST1_TAC) WSEG_WORDLEN
       THEN RESQ_IMP_RES_THEN (IMP_RES_THEN COND_REWRITE1_TAC) BIT_WSEG
       THENL[
-    	IMP_RES_TAC PRE_LESS_REFL,
+        IMP_RES_TAC PRE_LESS_REFL,
 
-    	CONV_TAC ((RAND_CONV o RATOR_CONV o RAND_CONV) (REWR_CONV ADD_SYM))
+        CONV_TAC ((RAND_CONV o RATOR_CONV o RAND_CONV) (REWR_CONV ADD_SYM))
         THEN PURE_ONCE_REWRITE_TAC[PRE_SUB1]
         THEN REFL_TAC
            ],
@@ -459,32 +489,36 @@ val SHL_WSEG = store_thm("SHL_WSEG",
       THEN TRY REFL_TAC THENL[
         RESQ_IMP_RES_THEN (IMP_RES_THEN SUBST1_TAC) WSEG_WORDLEN
         THEN PURE_ONCE_REWRITE_TAC[PRE_SUB1]
-    	THEN RESQ_REWRITE1_TAC WSEG_WSEG THENL[
-    	  ARITH_TAC,
-    	  REWRITE_TAC[ADD_0]],
-    	RESQ_REWRITE1_TAC WSEG_WSEG THENL[
-    	  ARITH_TAC,
-    	  REWRITE_TAC[ADD_0]],
+        THEN RESQ_REWRITE1_TAC WSEG_WSEG THENL[
+          ARITH_TAC,
+          REWRITE_TAC[ADD_0]],
+        RESQ_REWRITE1_TAC WSEG_WSEG THENL[
+          ARITH_TAC,
+          REWRITE_TAC[ADD_0]],
 
         RESQ_IMP_RES_THEN (IMP_RES_THEN SUBST1_TAC) WSEG_WORDLEN
         THEN PURE_ONCE_REWRITE_TAC[PRE_SUB1]
-    	THEN RESQ_REWRITE1_TAC WSEG_WSEG THENL[
-    	  ARITH_TAC,
-    	  REWRITE_TAC[ADD_0]]]]
+        THEN RESQ_REWRITE1_TAC WSEG_WSEG THENL[
+          ARITH_TAC,
+          REWRITE_TAC[ADD_0]]]]
    end);
 
 (* |- !n. !w :: PWORDLEN n.
      !m k. (m + k) <= n ==> 0 < m ==>
       (!b. SHL F(WSEG m k w)b = BIT(k + (m - 1))w,WCAT(WSEG(m - 1)k w,WORD[b])) *)
 val SHL_WSEG_1F = save_thm("SHL_WSEG_1F",
-    let val th1 = SPEC_ALL(RESQ_SPEC_ALL(SPEC_ALL SHL_WSEG))
+    let val th1 = RESQ_SPECL [``n : num``, ``w : 'a word``, ``m : num``, ``k : num``] SHL_WSEG
     val {Rator = P, Rand = v} = dest_comb(hd(hyp th1))
     val ante = fst(strip_imp(concl th1))
-    val th2 = CONV_RULE(ONCE_DEPTH_CONV COND_CONV)
-    	(SPEC (--`F`--) (UNDISCH_ALL th1))
+    val th2 = SPEC ``b : 'a`` (CONV_RULE(ONCE_DEPTH_CONV COND_CONV)
+        (SPEC (--`F`--) (UNDISCH_ALL th1)))
     in
-    GEN_ALL(RESQ_GEN (v,P) (GENL[(--`m:num`--),(--`k:num`--)]
-                                (itlist DISCH ante th2)))
+    GEN_ALL
+    (CONV_RULE (HO_REWR_CONV (GSYM RES_FORALL))
+     (GEN ``w : 'a word``
+      (DISCH_ALL
+       (GENL[``b : 'a``, (--`m:num`--),(--`k:num`--)]
+        (itlist DISCH ante th2)))))
     end);
 
 
@@ -521,7 +555,7 @@ val WSEG_SHL = store_thm("WSEG_SHL",
         RESQ_IMP_RES_THEN MATCH_MP_TAC WSEG_PWORDLEN
         THEN CONV_TAC (ONCE_DEPTH_CONV num_CONV)
         THEN REWRITE_TAC[ADD,LESS_EQ_MONO,ZERO_LESS_EQ],
-    	MATCH_ACCEPT_TAC PWORDLEN1],
+        MATCH_ACCEPT_TAC PWORDLEN1],
       ARITH_TAC,
       CONV_TAC (ONCE_DEPTH_CONV num_CONV) THEN IMP_RES_TAC LESS_OR,
       RESQ_REWRITE1_TAC WSEG_WSEG THENL[
