src/word/theories/bword_arithScript.sml
@@ -1,25 +1,28 @@
 (*-----------------------------------------------------------------------*)
-(* FILE: bword_arith.ml	DATE: 15 Jan 93					 *)
-(* WRITES: bword_arith.th    	    					 *)
-(* TRANSLATOR: Paul Curzon  3 June 1993, Sept 1994			 *)
-(* This theory contains defintions and theorems on boolean word 	 *)
-(* arithmetic, e.g. addition.	    					 *)
+(* FILE: bword_arith.ml DATE: 15 Jan 93                                  *)
+(* WRITES: bword_arith.th                                                *)
+(* TRANSLATOR: Paul Curzon  3 June 1993, Sept 1994                       *)
+(* UPDATED for new res_quan theories by Joe Hurd, November 2001          *)
+(* This theory contains defintions and theorems on boolean word          *)
+(* arithmetic, e.g. addition.                                            *)
 (*-----------------------------------------------------------------------*)
 
 
 open HolKernel Parse boolLib Prim_rec numLib res_quanLib;
 open rich_listTheory pairTheory arithmeticTheory prim_recTheory numTheory;
-open Cond_rewrite Res_quan;
+open Cond_rewrite;
 open word_baseTheory word_numTheory bword_numTheory;
 open Base;
+open res_quanTheory bossLib pred_setTheory;
 
-infix THEN THENL THENC ORELSE ORELSEC;
+infix THEN THENL THENC ORELSE ORELSEC |->;
 
-val _ = new_theory"bword_arith";
+val _ = new_theory "bword_arith";
 
+val GGEN_TAC = RESQ_GEN_TAC ORELSE GEN_TAC;
 
 (*-----------------------------------------------------------------------*)
-(* We begin with with lemmas about arithmetic of natural numbers.	 *)
+(* We begin with with lemmas about arithmetic of natural numbers.        *)
 (* They are used to proof the interesting theorems about word arithmetic *)
 (*-----------------------------------------------------------------------*)
 
@@ -28,7 +31,7 @@ val MULT_LEFT_1 = GEN_ALL (el 3 (CONJ_LIST 6 (SPEC_ALL MULT_CLAUSES)));
 val ADD_DIV_SUC_DIV = prove(
     (--`!n. 0 < n ==> !r. (((n + r) DIV n) = SUC (r DIV n))`--),
     let val MULT_LEM = SYM (PURE_ONCE_REWRITE_RULE[ADD_SYM]
-    	(el 5 (CONJ_LIST 6 (SPECL[(--`q:num`--),(--`n:num`--)] MULT_CLAUSES)))) in
+        (el 5 (CONJ_LIST 6 (SPECL[(--`q:num`--),(--`n:num`--)] MULT_CLAUSES)))) in
     CONV_TAC (ONCE_DEPTH_CONV RIGHT_IMP_FORALL_CONV)
     THEN REPEAT GEN_TAC THEN ASM_CASES_TAC (--`r < n`--) THENL[
       IMP_RES_THEN SUBST1_TAC LESS_DIV_EQ_ZERO THEN DISCH_TAC
@@ -55,9 +58,9 @@ val LESS_MONO_DIV = prove(
     CONV_TAC (REDEPTH_CONV RIGHT_IMP_FORALL_CONV)
     THEN REPEAT GEN_TAC THEN DISCH_TAC
     THEN DISCH_THEN ((CHOOSE_THEN (CONJUNCTS_THEN2 SUBST_ALL_TAC ASSUME_TAC)) o
-    	(MATCH_MP Less_lemma))
+        (MATCH_MP Less_lemma))
     THEN REPEAT_TCL CHOOSE_THEN (CONJUNCTS_THEN2 SUBST1_TAC ASSUME_TAC)
-    	(SPEC (--`p:num`--) (MATCH_MP DA (ASSUME (--`0 < n`--))))
+        (SPEC (--`p:num`--) (MATCH_MP DA (ASSUME (--`0 < n`--))))
     THEN IMP_RES_THEN (fn t => REWRITE_TAC[t]) DIV_MULT
     THEN PURE_ONCE_REWRITE_TAC[GSYM ADD_ASSOC]
     THEN IMP_RES_TAC ADD_DIV_ADD_DIV
@@ -68,7 +71,7 @@ val LESS_EQ_MONO_DIV = prove(
     CONV_TAC (REDEPTH_CONV RIGHT_IMP_FORALL_CONV)
     THEN REPEAT GEN_TAC THEN DISCH_TAC
     THEN DISCH_THEN (fn t =>  DISJ_CASES_THEN2 ASSUME_TAC SUBST1_TAC
-    	(REWRITE_RULE[LESS_OR_EQ]t)) THENL[
+        (REWRITE_RULE[LESS_OR_EQ]t)) THENL[
      IMP_RES_TAC LESS_MONO_DIV,
      REWRITE_TAC[LESS_EQ_REFL]]);
 
@@ -95,9 +98,9 @@ val ADD_MONO_EQ = ARITH_PROVE (--`!m n p. ((p + m) = (p + n)) = (m = n)`--);
 
 
 (*-----------------------------------------------------------------------*)
-(* ACARRY n w1 w2 cin is the carry input at position n. It is		*)
-(* defined in terms of addition of the bits --- classic definition of	*)
-(* ripple carry.	    	    	    				*)
+(* ACARRY n w1 w2 cin is the carry input at position n. It is           *)
+(* defined in terms of addition of the bits --- classic definition of   *)
+(* ripple carry.                                                        *)
 (*-----------------------------------------------------------------------*)
 
 val ACARRY_DEF = new_recursive_definition {
@@ -108,13 +111,13 @@ val ACARRY_DEF = new_recursive_definition {
    (ACARRY 0 w1 w2 cin = (cin:bool)) /\
    (ACARRY (SUC n) w1 w2 cin =
       VB(((BV (BIT n w1)) + (BV (BIT n w2)) +
-    	  (BV (ACARRY n w1 w2 cin))) DIV 2))
+          (BV (ACARRY n w1 w2 cin))) DIV 2))
  `--
  };
 
 (*-----------------------------------------------------------------------*)
 (* ICARRY n w1 w1 cin is the implementation of ripple carry using logic  *)
-(* gates only, i.e. /\, \/ only.	    				*)
+(* gates only, i.e. /\, \/ only.                                        *)
 (*-----------------------------------------------------------------------*)
 
 val ICARRY_DEF = new_recursive_definition {
@@ -131,24 +134,24 @@ val ICARRY_DEF = new_recursive_definition {
 
 (*-----------------------------------------------------------------------*)
 (* We now prove that the implementation of ripple carry is equivalent to *)
-(* the specification for all position k less the the word size,		*)
-(* i.e. ACARRY_EQ_ICARRY						*)
+(* the specification for all position k less the the word size,         *)
+(* i.e. ACARRY_EQ_ICARRY                                                *)
 (*-----------------------------------------------------------------------*)
 
 val div_mod_lemmas =
     let val lm = prove((--`2 + x = SUC(SUC x)`--),
-    	CONV_TAC (REDEPTH_CONV num_CONV) THEN REWRITE_TAC[ADD_CLAUSES])
+        CONV_TAC (REDEPTH_CONV num_CONV) THEN REWRITE_TAC[ADD_CLAUSES])
     val less2 = SUBS[SYM (num_CONV (--`2`--))](SPEC (--`1`--) LESS_0)
     val less21 = SUBS[SYM (REDEPTH_CONV num_CONV (--`2`--))]
         (SPEC (--`SUC 0`--) LESS_SUC_REFL)
     val div22 = GEN_ALL(SUBS[lm]
-    	(SPEC (--`x:num`--)(MP (SPEC (--`2`--) ADD_DIV_SUC_DIV) less2)))
+        (SPEC (--`x:num`--)(MP (SPEC (--`2`--) ADD_DIV_SUC_DIV) less2)))
     val div21 =
           MP (SPECL[(--`SUC 0`--), (--`2`--)] LESS_DIV_EQ_ZERO) less21
     val div20 = MP (SPEC (--`2`--) ZERO_DIV) less2
-    val	mod20 = MP (SPEC (--`2`--) ZERO_MOD) less2
-    val	mod21 = REWRITE_RULE[MULT,ADD]
-    	    (SPEC (--`0`--)
+    val mod20 = MP (SPEC (--`2`--) ZERO_MOD) less2
+    val mod21 = REWRITE_RULE[MULT,ADD]
+            (SPEC (--`0`--)
                  (MP (SPECL [(--`2`--), (--`SUC 0`--)] MOD_MULT) less21))
    in
     [div22,div21,div20,mod21,mod20]
@@ -158,8 +161,8 @@ val ACARRY_EQ_ICARRY = store_thm("ACARRY_EQ_ICARRY",
     (--`!n. !w1 w2::PWORDLEN n. !cin k. k <= n ==>
      (ACARRY k w1 w2 cin = ICARRY k w1 w2 cin)`--),
     let val lem1 = GEN_ALL (IMP_TRANS
-    	(snd(EQ_IMP_RULE(SPEC_ALL LESS_EQ)))
-    	(SPEC_ALL LESS_IMP_LESS_OR_EQ))
+        (snd(EQ_IMP_RULE(SPEC_ALL LESS_EQ)))
+        (SPEC_ALL LESS_IMP_LESS_OR_EQ))
     in
     GEN_TAC THEN REPEAT RESQ_GEN_TAC
     THEN GEN_TAC THEN INDUCT_TAC THEN DISCH_TAC
@@ -168,19 +171,19 @@ val ACARRY_EQ_ICARRY = store_thm("ACARRY_EQ_ICARRY",
     THEN IMP_RES_TAC lem1 THEN RES_TAC
     THEN PURE_ONCE_ASM_REWRITE_TAC[]
     THEN MAP_EVERY BOOL_CASES_TAC [(--`BIT k (w1:bool word)`--),
-    	(--`BIT k (w2:bool word)`--), (--`ICARRY k w1 w2 cin`--)]
+        (--`BIT k (w2:bool word)`--), (--`ICARRY k w1 w2 cin`--)]
     THEN REWRITE_TAC([ADD_CLAUSES,NOT_SUC,SUC_NOT] @ div_mod_lemmas)
    end);
 
 (*-----------------------------------------------------------------------*)
-(*   	    Word Addition   	    					*)
+(*          Word Addition                                               *)
 (* We now develop a theory about word addition. The addition of two n-bit*)
-(* words can be carried out in two different ways:			*)
-(* 1) convert the operands into natural numbers and do addition (+),	*)
-(* 2) split the operands into segments, then using method 1 to add the	*)
+(* words can be carried out in two different ways:                      *)
+(* 1) convert the operands into natural numbers and do addition (+),    *)
+(* 2) split the operands into segments, then using method 1 to add the  *)
 (*    corresponding segments as they were smaller words, then concatenate*)
-(*    the sums to form the final result.					*)
-(* We need to prove that these two methods give the same results.	*)
+(*    the sums to form the final result.                                        *)
+(* We need to prove that these two methods give the same results.       *)
 (*-----------------------------------------------------------------------*)
 
 (* We need a series of lemmas starting here
@@ -212,18 +215,12 @@ val LESS_EQ1_LESS2 = REWRITE_RULE[Less2,PRE]
     (CONV_RULE ((RAND_CONV o RAND_CONV o RAND_CONV o RAND_CONV)num_CONV)
      (SPECL [(--`n:num`--),(--`2`--)] LESS_IMP_LESS_EQ_PRE));
 
-(* BNVAL_LESS_EQ =
-    |- !n. !w :: PWORDLEN n. (BNVAL w) <= ((2 EXP n) - 1) *)
-
-val BNVAL_LESS_EQ =
-    GEN_ALL (RESQ_GEN_ALL (PURE_ONCE_REWRITE_RULE[PRE_SUB1]
-    (EQ_MP
-      (SPEC (--`BNVAL w`--)
-(*       (GEN  (--`m:num`--)*)
-       (MATCH_MP LESS_IMP_LESS_EQ_PRE
-     	(SUBS[SYM (num_CONV (--`2`--))]
-             (SPECL [(--`n:num`--), (--`1`--)] ZERO_LESS_EXP) )))
-      (GQSPEC_ALL BNVAL_MAX))));
+val BNVAL_LESS_EQ = store_thm
+  ("BNVAL_LESS_EQ",
+   ``!n. !w :: PWORDLEN n. (BNVAL w) <= ((2 EXP n) - 1)``,
+   REPEAT RESQ_STRIP_TAC
+   THEN MP_TAC (RESQ_SPECL [``n : num``, ``w : bool word``] BNVAL_MAX)
+   THEN DECIDE_TAC);
 
 val ADD_BNVAL_LESS_EQ = prove(
     (--`!n. !w1 w2::PWORDLEN n. !cin.
@@ -231,11 +228,11 @@ val ADD_BNVAL_LESS_EQ = prove(
     let val LESS_EQ_SUB_ADD =
        ARITH_PROVE (--`!m n p. (p <= m) ==> ((m - p) + n = (m + n) - p)`--)
     val [t1,t2] = map (fn t => RESQ_SPEC t (SPEC_ALL BNVAL_LESS_EQ))
-    	 [(--`w1:bool word`--), (--`w2:bool word`--)]
+         [(--`w1:bool word`--), (--`w2:bool word`--)]
     val lem = PURE_REWRITE_RULE[GSYM TIMES2,LEFT_SUB_DISTRIB,MULT_CLAUSES]
-    	(MATCH_MP LESS_EQ_LESS_EQ_MONO (CONJ t1 t2))
+        (MATCH_MP LESS_EQ_LESS_EQ_MONO (CONJ t1 t2))
     val lem2 = (MATCH_MP LESS_EQ_LESS_EQ_MONO
-    	(CONJ lem (SPEC (--`cin:bool`--)  BV_LESS_EQ_1)))
+        (CONJ lem (SPEC (--`cin:bool`--)  BV_LESS_EQ_1)))
     in
     REPEAT GGEN_TAC THEN PURE_ONCE_REWRITE_TAC[ADD_ASSOC,EXP]
     THEN MP_TAC lem2 THEN COND_REWRITE1_TAC LESS_EQ_SUB_ADD THENL[
@@ -244,7 +241,7 @@ val ADD_BNVAL_LESS_EQ = prove(
      THEN CONV_TAC (ONCE_DEPTH_CONV num_CONV)
      THEN REWRITE_TAC[GSYM LESS_EQ, ZERO_LESS_EXP],
      PURE_ONCE_REWRITE_TAC[GSYM ADD1]
-     THEN CONV_TAC ((LHS_CONV o RHS_CONV o RHS_CONV)num_CONV)
+     THEN CONV_TAC ((LAND_CONV o RAND_CONV o RAND_CONV)num_CONV)
      THEN REWRITE_TAC[SUB_MONO_EQ]]
     end);
 
@@ -259,22 +256,22 @@ val EXP_SUB1_LESS = prove((--`((2 EXP n) - 1) < (2 EXP n)`--),
     THEN MATCH_ACCEPT_TAC ZERO_LESS_TWO_EXP);
 
 
-(* ADD_BNVAL_LESS_EQ1 =
-    |- !n cin.
-       !w1 w2 :: PWORDLEN n.
-     (((BNVAL w1) + ((BNVAL w2) + (BV cin))) DIV (2 EXP n)) <= (SUC 0) *)
-
-val ADD_BNVAL_LESS_EQ1 =
-  let val LESS_EQ_ADD_SUB1 = ARITH_PROVE (--`!m n p. (p <= n) ==>
-    	(m + (n - p) = (m + n) - p)`--)
+val ADD_BNVAL_LESS_EQ1 = store_thm
+  ("ADD_BNVAL_LESS_EQ1",
+   ``!n cin. !w1 w2 :: PWORDLEN n.
+       (((BNVAL w1) + ((BNVAL w2) + (BV cin))) DIV (2 EXP n)) <= (SUC 0)``,
+  let
+    val LESS_EQ_ADD_SUB1 = ARITH_PROVE (--`!m n p. (p <= n) ==>
+                                        (m + (n - p) = (m + n) - p)`--)
     val ONE_LESS_EQ_TWO_EXP =
-    	REWRITE_RULE[LESS_EQ,GSYM(num_CONV(--`1`--))]ZERO_LESS_TWO_EXP
+      REWRITE_RULE[LESS_EQ,GSYM(num_CONV(--`1`--))]ZERO_LESS_TWO_EXP
     val lm1 = SYM (SPECL[(--`n:num`--), (--`2 EXP n`--)]
-        (GEN(--`m:num`--)
-    	 (MATCH_MP LESS_EQ_ADD_SUB1 (SPEC_ALL ONE_LESS_EQ_TWO_EXP))))
+                   (GEN(--`m:num`--)
+                    (MATCH_MP LESS_EQ_ADD_SUB1 (SPEC_ALL ONE_LESS_EQ_TWO_EXP))))
   in
-  GENL[(--`n:num`--),(--`cin:bool`--)]
-   (RESQ_GEN_ALL (PROVE_HYP (SPEC_ALL ZERO_LESS_TWO_EXP)
+    REPEAT RESQ_STRIP_TAC
+    THEN MP_TAC
+  (PROVE_HYP (SPEC_ALL ZERO_LESS_TWO_EXP)
    (CONV_RULE ((RAND_CONV o RAND_CONV)
         (COND_REWRITE1_CONV [EXP_SUB1_LESS] LESS_DIV_EQ_ZERO))
     (CONV_RULE (RAND_CONV
@@ -286,90 +283,93 @@ val ADD_BNVAL_LESS_EQ1 =
               (SPEC (--`2 EXP n`--) LESS_EQ_MONO_DIV)
               (SPEC(--`n:num`--) ZERO_LESS_TWO_EXP)
               )
-        (SUBS[lm1](REWRITE_RULE[EXP,TIMES2](GQSPEC_ALL ADD_BNVAL_LESS_EQ)))
-     )))
-     ))))
-  end;
+        (SUBS[lm1](REWRITE_RULE[EXP,TIMES2](RESQ_SPECL [``n : num``, ``w1 : bool word``, ``w2 : bool word``, ``cin : bool``] ADD_BNVAL_LESS_EQ))))
+     ))
+   )))
+    THEN PROVE_TAC [ADD_ASSOC]
+  end);
 
-(* ADD_BV_BNVAL_DIV_LESS_EQ1 =
-|- !n x1 x2 cin.
-    !w1 w2 :: PWORDLEN n.
+val ADD_BV_BNVAL_DIV_LESS_EQ1 = store_thm
+  ("ADD_BV_BNVAL_DIV_LESS_EQ1",
+   ``!n x1 x2 cin. !w1 w2 :: PWORDLEN n.
      ((((BV x1) + (BV x2)) +
-       (((BNVAL w1) + ((BNVAL w2) + (BV cin))) DIV (2 EXP n))) DIV 2) <= 1 *)
-
-val ADD_BV_BNVAL_DIV_LESS_EQ1 =
-    GENL[(--`n:num`--),(--`x1:bool`--),(--`x2:bool`--),(--`cin:bool`--)]
-    (RESQ_GEN_ALL (SUBS[SYM (num_CONV (--`1`--))]
+       (((BNVAL w1) + ((BNVAL w2) + (BV cin))) DIV (2 EXP n))) DIV 2) <= 1``,
+   REPEAT RESQ_STRIP_TAC
+   THEN MP_TAC
      (CONV_RULE ((RAND_CONV o RAND_CONV)
-    	(COND_REWRITE1_CONV [Less2_SUC0] LESS_DIV_EQ_ZERO))
+        (COND_REWRITE1_CONV [Less2_SUC0] LESS_DIV_EQ_ZERO))
       (CONV_RULE (RAND_CONV
-    	(COND_REWRITE1_CONV [Less2] ADD_DIV_SUC_DIV))
+        (COND_REWRITE1_CONV [Less2] ADD_DIV_SUC_DIV))
        (MATCH_MP (MATCH_MP LESS_EQ_MONO_DIV Less2)
         (MATCH_MP LESS_EQ_LESS_EQ_MONO (CONJ (SPEC_ALL ADD_BV_LESS_EQ_2)
-    	(GQSPEC_ALL ADD_BNVAL_LESS_EQ1))))))));
+        (Q_RESQ_SPECL [`n`, `cin`, `w1`, `w2`] ADD_BNVAL_LESS_EQ1))))))
+   THEN PROVE_TAC [ONE]);
 
-(* ADD_BV_BNVAL_LESS_EQ =
-|- !n x1 x2 cin.
-    !w1 w2 :: PWORDLEN n.
-     (((BV x1) + (BV x2)) + ((BNVAL w1) + ((BNVAL w2) + (BV cin)))) <=
-     (SUC(2 EXP (SUC n))) *)
+val ADD_BV_BNVAL_LESS_EQ = store_thm
+  ("ADD_BV_BNVAL_LESS_EQ",
+   ``!n x1 x2 cin. !w1 w2 :: PWORDLEN n.
+       (((BV x1) + (BV x2)) + ((BNVAL w1) + ((BNVAL w2) + (BV cin)))) <=
+       (SUC(2 EXP (SUC n)))``,
+   REPEAT RESQ_STRIP_TAC
+   THEN MP_TAC
+     (let val lm = MATCH_MP SUC_PRE (MATCH_MP SUC_LESS
+        (CONV_RULE (LAND_CONV num_CONV) (SPEC_ALL ONE_LESS_TWO_EXP_SUC)))
+     in
+       REWRITE_RULE[GSYM PRE_SUB1,ADD,lm]
+       (CONV_RULE ((RAND_CONV o LAND_CONV)(REDEPTH_CONV num_CONV))
+        (MATCH_MP LESS_EQ_LESS_EQ_MONO
+         (CONJ (SPEC_ALL ADD_BV_LESS_EQ_2) (Q_RESQ_SPECL [`n`, `w1`, `w2`, `cin`] ADD_BNVAL_LESS_EQ))))
+     end)
+   THEN PROVE_TAC [ADD_ASSOC]);
 
-val ADD_BV_BNVAL_LESS_EQ =
-    let val lm = MATCH_MP SUC_PRE (MATCH_MP SUC_LESS
-    	(CONV_RULE (LHS_CONV num_CONV) (SPEC_ALL ONE_LESS_TWO_EXP_SUC)))
-    in
-    GENL[(--`n:num`--),(--`x1:bool`--),(--`x2:bool`--),(--`cin:bool`--)]
-     (RESQ_GEN_ALL
-    (REWRITE_RULE[GSYM PRE_SUB1,ADD,lm]
-    (CONV_RULE ((RAND_CONV o LHS_CONV)(REDEPTH_CONV num_CONV))
-    (MATCH_MP LESS_EQ_LESS_EQ_MONO
-    (CONJ (SPEC_ALL ADD_BV_LESS_EQ_2) (GQSPEC_ALL ADD_BNVAL_LESS_EQ))))))
-    end;
-
-(* ADD_BV_BNVAL_LESS_EQ1 =
-|- !n x1 x2 cin. !w1 w2 :: PWORDLEN n.
- ((((BV x1) + (BV x2)) + ((BNVAL w1) + ((BNVAL w2) + (BV cin)))) DIV
-  (2 EXP (SUC n))) <= 1 *)
-
-val ADD_BV_BNVAL_LESS_EQ1 =
-  (GENL[(--`n:num`--),(--`x1:bool`--),(--`x2:bool`--),(--`cin:bool`--)] o
-     RESQ_GEN_ALL)
-  (SUBS[SYM (SPEC_ALL ADD1)]
-   (PROVE_HYP (MATCH_MP SUC_LESS
-    	(CONV_RULE (LHS_CONV num_CONV) (SPEC_ALL ONE_LESS_TWO_EXP_SUC)))
-    (SUBS[(REWRITE_RULE[MULT_LEFT_1,ADD1]
-    	  (SPEC (--`1`--) (MATCH_MP DIV_MULT(SPEC_ALL ONE_LESS_TWO_EXP_SUC))))]
-    	(PURE_REWRITE_RULE[ADD1] (MATCH_MP
-    	 (GEN_ALL(UNDISCH (SPEC_ALL(SPEC (--`2 EXP (SUC n)`--) LESS_EQ_MONO_DIV))))
-    	  (GQSPEC_ALL ADD_BV_BNVAL_LESS_EQ))))));
+val ADD_BV_BNVAL_LESS_EQ1 = store_thm
+  ("ADD_BV_BNVAL_LESS_EQ1",
+   ``!n x1 x2 cin. !w1 w2 :: PWORDLEN n.
+       ((((BV x1) + (BV x2)) + ((BNVAL w1) + ((BNVAL w2) + (BV cin)))) DIV
+       (2 EXP (SUC n))) <= 1``,
+   REPEAT RESQ_STRIP_TAC
+   THEN MP_TAC
+   (SUBS[SYM (SPEC_ALL ADD1)]
+    (PROVE_HYP
+     (MATCH_MP SUC_LESS
+      (CONV_RULE (LAND_CONV num_CONV) (SPEC_ALL ONE_LESS_TWO_EXP_SUC)))
+     (SUBS
+      [(REWRITE_RULE[MULT_LEFT_1,ADD1]
+        (SPEC (--`1`--) (MATCH_MP DIV_MULT(SPEC_ALL ONE_LESS_TWO_EXP_SUC))))]
+      (PURE_REWRITE_RULE[ADD1]
+       (MATCH_MP
+        (GEN_ALL
+         (UNDISCH(SPEC_ALL(SPEC (--`2 EXP (SUC n)`--) LESS_EQ_MONO_DIV))))
+        (Q_RESQ_SPECL [`n`, `x1`, `x2`, `cin`, `w1`, `w2`]
+         ADD_BV_BNVAL_LESS_EQ))))))
+   THEN PROVE_TAC [ADD_ASSOC, ADD1]);
 
 (* seg_pw =
-    |- !w. PWORDLEN n w ==> (SUC k) <= n ==> PWORDLEN(SUC k)(WSEG(SUC k)0 w) *)
-
+|- !w. w IN PWORDLEN n ==> SUC k <= n ==> WSEG (SUC k) 0 w IN PWORDLEN(SUC k) *)
 val seg_pw = GEN (--`w:'a word`--) (DISCH_ALL
     (REWRITE_RULE[ADD_0] (SPECL[(--`SUC k`--),(--`0`--)]
-     (RESQ_SPEC_ALL (SPEC (--`n:num`--) WSEG_PWORDLEN))))) ;
+     (Q_RESQ_SPECL [`w`] (SPEC (--`n:num`--) WSEG_PWORDLEN)))));
 
 (* bit_thm =
 |- !w.
-    PWORDLEN n w ==> (SUC k) <= n ==> (BIT k(WSEG(SUC k)0 w) = BIT k w) *)
-
+    w IN PWORDLEN n ==> SUC k <= n ==> (BIT k (WSEG(SUC k)0 w) = BIT k w) *)
 val bit_thm = GEN (--`w:'a word`--) (DISCH_ALL
     (REWRITE_RULE[ADD_CLAUSES,LESS_SUC_REFL]
-    (SPECL [(--`SUC k`--), (--`0`--),(--`k:num`--)](RESQ_SPEC_ALL(SPEC (--`n:num`--) BIT_WSEG)))));
+    (SPECL [(--`SUC k`--), (--`0`--),(--`k:num`--)]
+     (Q_RESQ_SPECL [`w`] (SPEC (--`n:num`--) BIT_WSEG)))));
 
 (* seg_thm =
-|- !w. PWORDLEN n w ==> (SUC k) <= n ==>
+|- !w. w IN PWORDLEN n ==> SUC k <= n ==>
     (WSEG k 0(WSEG(SUC k)0 w) = WSEG k 0 w) *)
-
 val seg_thm = GEN (--`w:'a word`--) (DISCH_ALL
     (REWRITE_RULE[ADD_CLAUSES,LESS_EQ_SUC_REFL]
-    (SPECL [(--`SUC k`--), (--`0`--),(--`k:num`--),(--`0`--)](RESQ_SPEC_ALL(SPEC (--`n:num`--) WSEG_WSEG)))));
+    (SPECL [(--`SUC k`--), (--`0`--),(--`k:num`--),(--`0`--)]
+     (Q_RESQ_SPECL [`w`] (SPEC (--`n:num`--) WSEG_WSEG)))));
 
 (* seg_pw_thm' = |- !w. PWORDLEN n w ==> k <= n ==> PWORDLEN k(WSEG k 0 w) *)
-
 val seg_pw_thm' = GEN (--`w:bool word`--) (DISCH_ALL (REWRITE_RULE[ADD_CLAUSES]
-    (GQSPECL [(--`n:num`--), (--`w:bool word`--), (--`k:num`--), (--`0`--)] WSEG_PWORDLEN)));
+    (RESQ_SPECL [(--`n:num`--), (--`w:bool word`--), (--`k:num`--), (--`0`--)]
+     (INST_TYPE [alpha |-> bool] WSEG_PWORDLEN))));
 
 fun spec_thm th =
      (map (fn t => UNDISCH_ALL(ISPEC t th)) [(--`w2:bool word`--), (--`w1:bool word`--)]);
@@ -392,16 +392,16 @@ PWORDLEN n w1, k <= n, PWORDLEN n w2
       (2 EXP k))) DIV 2) <= 1 *)
 
 val less1_lem = itlist PROVE_HYP (spec_thm seg_pw_thm')
-    (GQSPECL [(--`k:num`--), (--`BIT k (w1:bool word)`--),
+    (RESQ_SPECL [(--`k:num`--), (--`BIT k (w1:bool word)`--),
               (--`BIT k (w2:bool word)`--), (--`cin:bool`--),
               (--`WSEG k 0 (w1:bool word)`--), (--`WSEG k 0 (w2:bool word)`--)]
        ADD_BV_BNVAL_DIV_LESS_EQ1);
 
 (*-----------------------------------------------------------------------*)
-(* ACARRY_EQ_ADD_DIV 	    	    					*)
-(* We can now prove the ripple carry at position k (ACARRY k ...) is	*)
-(* equal to the arithmetic carry resulting from adding the lower-order	*)
-(* segments of the operands. 	    					*)
+(* ACARRY_EQ_ADD_DIV                                                    *)
+(* We can now prove the ripple carry at position k (ACARRY k ...) is    *)
+(* equal to the arithmetic carry resulting from adding the lower-order  *)
+(* segments of the operands.                                            *)
 (*-----------------------------------------------------------------------*)
 
 val ACARRY_EQ_ADD_DIV = store_thm("ACARRY_EQ_ADD_DIV",
@@ -416,7 +416,7 @@ val ACARRY_EQ_ADD_DIV = store_thm("ACARRY_EQ_ADD_DIV",
      THEN MAP_EVERY IMP_RES_TAC [LESS_IMP_LESS_OR_EQ,seg_pw]
      THEN SUBST1_TAC add_left
      THEN CONV_TAC ((RAND_CONV o RATOR_CONV o RAND_CONV)
-    	 (REWR_CONV (GSYM ADD_ASSOC)))
+         (REWR_CONV (GSYM ADD_ASSOC)))
      THEN PURE_ONCE_REWRITE_TAC[EXP]
      THEN CONV_TAC ((RAND_CONV o RAND_CONV)(REWR_CONV MULT_SYM))
      THEN COND_REWRITE1_TAC (GSYM DIV_DIV_DIV_MULT) THENL[
@@ -427,38 +427,38 @@ val ACARRY_EQ_ADD_DIV = store_thm("ACARRY_EQ_ADD_DIV",
       THEN COND_REWRITE1_TAC BV_VB THENL[
        PURE_ONCE_REWRITE_TAC[LESS_EQ1_LESS2]
        THEN IMP_RES_TAC LESS_IMP_LESS_OR_EQ
-       THEN MATCH_ACCEPT_TAC less1_lem,
+       THEN PROVE_TAC [ADD_ASSOC, less1_lem],
        PURE_ONCE_REWRITE_TAC[ADD_ASSOC] THEN REFL_TAC]]]);
 
 (*-----------------------------------------------------------------------*)
-(* The theorem asserting the equivalence ot the two addition methods.	*)
+(* The theorem asserting the equivalence ot the two addition methods.   *)
 (*-----------------------------------------------------------------------*)
 
 val ADD_WORD_SPLIT = store_thm("ADD_WORD_SPLIT",
     (--`!n1 n2. !w1 w2::PWORDLEN (n1 + n2). !cin.
      NBWORD (n1 + n2) ((BNVAL w1) + (BNVAL w2) + (BV cin)) =
      WCAT ((NBWORD n1 ((BNVAL (WSEG n1 n2 w1)) + (BNVAL (WSEG n1 n2 w2)) +
-    	    	       (BV (ACARRY n2 w1 w2 cin)))),
-    	   (NBWORD n2 ((BNVAL (WSEG n2 0 w1)) + (BNVAL (WSEG n2 0 w2)) +
-    	    	       (BV cin))))`--),
+                       (BV (ACARRY n2 w1 w2 cin)))),
+           (NBWORD n2 ((BNVAL (WSEG n2 0 w1)) + (BNVAL (WSEG n2 0 w2)) +
+                       (BV cin))))`--),
      let val lem1 = itlist (fn t1 => fn t2 => RESQ_MATCH_MP t2 t1)
-    	(map ASSUME [(--`PWORDLEN(n1 + (SUC n2))(w2:bool word)`--),
-    	    (--`PWORDLEN(n1 + (SUC n2))(w1:bool word)`--)])
-    	(SPECL[(--`n1:num`--), (--`SUC n2`--)] ADD_BNVAL_SPLIT)
+        (map ASSUME [(--`(w2:bool word) IN PWORDLEN(n1 + (SUC n2))`--),
+            (--`(w1:bool word) IN PWORDLEN(n1 + (SUC n2))`--)])
+        (SPECL[(--`n1:num`--), (--`SUC n2`--)] ADD_BNVAL_SPLIT)
      val wcat_11 =
          let val lm = (SPECL [(--`n1:num`--), (--`SUC n2`--)] WCAT_11)
-    	 val lms = map (fn t => SPECL t PWORDLEN_NBWORD)
-    	    [[(--`n1:num`--), (--`m11:num`--)],
+         val lms = map (fn t => SPECL t PWORDLEN_NBWORD)
+            [[(--`n1:num`--), (--`m11:num`--)],
              [(--`n1:num`--), (--`m12:num`--)],
-    	     [(--`SUC n2`--), (--`m21:num`--)],
+             [(--`SUC n2`--), (--`m21:num`--)],
              [(--`SUC n2`--), (--`m22:num`--)]]
          in
-    	  GENL[(--`m11:num`--), (--`m12:num`--),
+          GENL[(--`m11:num`--), (--`m12:num`--),
                (--`m21:num`--), (--`m22:num`--)]
-      	    (rev_itlist (fn t1 => fn t2 => RESQ_MATCH_MP t2 t1) lms lm)
+            (rev_itlist (fn t1 => fn t2 => RESQ_MATCH_MP t2 t1) lms lm)
         end
-     val acarry_lem = SPEC (--`SUC n2`--)(RESQ_SPEC_ALL
-    	  (SPEC (--`n1 + (SUC n2)`--) ACARRY_EQ_ADD_DIV))
+     val acarry_lem = SPEC (--`SUC n2`--)(Q_RESQ_SPECL [`w1`, `w2`]
+          (SPEC (--`n1 + (SUC n2)`--) ACARRY_EQ_ADD_DIV))
    in
     GEN_TAC THEN INDUCT_TAC THENL[
      REWRITE_TAC[ADD_0,NBWORD0,WCAT0,ACARRY_DEF]
@@ -473,40 +473,40 @@ val ADD_WORD_SPLIT = store_thm("ADD_WORD_SPLIT",
       PURE_ONCE_REWRITE_TAC[wcat_11] THEN CONJ_TAC THENL[
        CONV_TAC ((RAND_CONV o RAND_CONV)(REWR_CONV ADD_ASSOC))
        THEN DISJ_CASES_THEN2 SUBST1_TAC ASSUME_TAC
-    	   (SPEC (--`n1 = 0`--) EXCLUDED_MIDDLE) THENL[
-    	REWRITE_TAC[NBWORD0],
-    	IMP_RES_THEN (ASSUME_TAC o (SPEC (--`SUC n2`--)))
-    	  (PURE_ONCE_REWRITE_RULE[ADD_SYM] LESS_ADD_NONZERO)
+           (SPEC (--`n1 = 0`--) EXCLUDED_MIDDLE) THENL[
+        REWRITE_TAC[NBWORD0],
+        IMP_RES_THEN (ASSUME_TAC o (SPEC (--`SUC n2`--)))
+          (PURE_ONCE_REWRITE_RULE[ADD_SYM] LESS_ADD_NONZERO)
         THEN FIRST_ASSUM (SUBST1_TAC o (MATCH_MP acarry_lem))
-    	THEN REWRITE_TAC[ADD_ASSOC]],
-       CONV_TAC (LHS_CONV (REWR_CONV (GSYM NBWORD_MOD)))
+        THEN REWRITE_TAC[ADD_ASSOC]],
+       CONV_TAC (LAND_CONV (REWR_CONV (GSYM NBWORD_MOD)))
        THEN COND_REWRITE1_TAC MOD_TIMES
        THEN PURE_ONCE_REWRITE_TAC[ADD_ASSOC]
        THEN MATCH_ACCEPT_TAC NBWORD_MOD]]]
     end);
 
 (*-----------------------------------------------------------------------*)
-(* This theorem states the fact about taking a segment of the sum of	*)
-(* two words.	    	    	    					*)
+(* This theorem states the fact about taking a segment of the sum of    *)
+(* two words.                                                           *)
 (*-----------------------------------------------------------------------*)
 
 val WSEG_NBWORD_ADD = store_thm("WSEG_NBWORD_ADD",
     (--`!n. !w1 w2::PWORDLEN n. !m k cin. (m + k) <= n ==>
     (WSEG m k(NBWORD n ((BNVAL w1) + (BNVAL w2) + (BV cin))) =
      NBWORD m ((BNVAL (WSEG m k w1)) + (BNVAL (WSEG m k w2)) +
-    	       (BV(ACARRY k w1 w2 cin))))`--),
-    let val lem1 = RESQ_SPEC_ALL (CONV_RULE (COND_REWRITE1_CONV [] SUB_ADD)
-    	(SPECL[(--`n - k`--), (--`k:num`--)] ADD_WORD_SPLIT))
+               (BV(ACARRY k w1 w2 cin))))`--),
+    let val lem1 = Q_RESQ_SPECL [`w1`, `w2`] (CONV_RULE (COND_REWRITE1_CONV [] SUB_ADD)
+        (SPECL[(--`n - k`--), (--`k:num`--)] ADD_WORD_SPLIT))
     val lem2 = REWRITE_RULE[SUB_EQUAL_0,LESS_EQ_REFL]
                 (ISPECL[(--`n-k`--),(--`k:num`--),
                       (--`w1:bool word`--),(--`w2:bool word`--),
-    	(--`m:num`--),(--`k:num`--)](RESQ_REWR_CANON WSEG_WCAT_WSEG1))
+        (--`m:num`--),(--`k:num`--)](RESQ_REWR_CANON WSEG_WCAT_WSEG1))
     val lem3 = (CONV_RULE (COND_REWRITE1_CONV [] SUB_ADD)
-    	(SPECL[(--`(n-k)-m`--), (--`m:num`--)] ADD_WORD_SPLIT))
+        (SPECL[(--`(n-k)-m`--), (--`m:num`--)] ADD_WORD_SPLIT))
     val PW_WSEG_TAC =
-    	RESQ_IMP_RES_TAC WSEG_PWORDLEN THEN FIRST_ASSUM MATCH_MP_TAC
+        RESQ_IMP_RES_TAC WSEG_PWORDLEN THEN FIRST_ASSUM MATCH_MP_TAC
         THEN COND_REWRITE1_TAC SUB_ADD
-    	THEN MATCH_ACCEPT_TAC LESS_EQ_REFL
+        THEN MATCH_ACCEPT_TAC LESS_EQ_REFL
    in
     GEN_TAC THEN REPEAT RESQ_GEN_TAC THEN REPEAT GEN_TAC
     THEN DISCH_TAC THEN IMP_RES_TAC LESS_EQ_SPLIT
@@ -534,9 +534,9 @@ val ADD_NBWORD_EQ0_SPLIT = store_thm("ADD_NBWORD_EQ0_SPLIT",
      (NBWORD (n1+n2) ((BNVAL w1) + (BNVAL w2) + (BV cin)) = NBWORD (n1+n2) 0)
      =
      ((NBWORD n1 ((BNVAL (WSEG n1 n2 w1)) + (BNVAL (WSEG n1 n2 w2)) +
-    	    	(BV (ACARRY n2 w1 w2 cin))) = NBWORD n1 0) /\
+                (BV (ACARRY n2 w1 w2 cin))) = NBWORD n1 0) /\
       (NBWORD n2 ((BNVAL (WSEG n2 0 w1)) + (BNVAL (WSEG n2 0 w2)) +
-    	    	(BV cin)) = NBWORD n2 0))`--),
+                (BV cin)) = NBWORD n2 0))`--),
     REPEAT GEN_TAC THEN REPEAT RESQ_GEN_TAC THEN GEN_TAC
     THEN RESQ_REWRITE1_TAC ADD_WORD_SPLIT
     THEN RESQ_REWRITE1_TAC NBWORD_SPLIT
@@ -546,8 +546,8 @@ val ADD_NBWORD_EQ0_SPLIT = store_thm("ADD_NBWORD_EQ0_SPLIT",
      THEN ((MATCH_ACCEPT_TAC PWORDLEN_NBWORD) ORELSE REFL_TAC)]);
 
 (*-----------------------------------------------------------------------*)
-(* The theorem ACARRY_MSB states the value of the carry at the most 	*)
-(* significant position.	    	    					*)
+(* The theorem ACARRY_MSB states the value of the carry at the most     *)
+(* significant position.                                                        *)
 (*-----------------------------------------------------------------------*)
 
 val VB_MOD_2 = prove((--`!n. VB(n MOD 2) = VB n`--),
@@ -560,17 +560,17 @@ val ACARRY_MSB = store_thm("ACARRY_MSB",
      ACARRY n w1 w2 cin =
      BIT n (NBWORD (SUC n) ((BNVAL w1) + (BNVAL w2) + (BV cin)))`--),
     let val bit_lem = GEN_ALL
-    	(itlist PROVE_HYP
-    	 [(ISPEC (--`x:bool`--) PWORDLEN1),
+        (itlist PROVE_HYP
+         [(ISPEC (--`x:bool`--) PWORDLEN1),
               (SPECL [(--`SUC n`--),(--`m:num`--)] PWORDLEN_NBWORD)]
          (REWRITE_RULE[LESS_EQ_REFL,SUB_EQUAL_0,LESS_ADD_SUC,BIT0]
-    	  (PURE_ONCE_REWRITE_RULE[ADD_SYM](SUBS[num_CONV (--`1`--)]
-       	   (GQSPECL [(--`1`--),(--`SUC n`--),(--`WORD[x:bool]`--),
+          (PURE_ONCE_REWRITE_RULE[ADD_SYM](SUBS[num_CONV (--`1`--)]
+           (RESQ_SPECL [(--`1`--),(--`SUC n`--),(--`WORD[x:bool]`--),
                      (--`NBWORD (SUC n) m`--), (--`SUC n`--)]
-    	    BIT_WCAT_FST)))))
-    val lem1 = MP (GQSPECL [(--`SUC n`--), (--`w1:bool word`--),
+            (INST_TYPE [alpha |-> bool] BIT_WCAT_FST))))))
+    val lem1 = MP (RESQ_SPECL [(--`SUC n`--), (--`w1:bool word`--),
                             (--`w2:bool word`--),(--`n:num`--)]
-    	      ACARRY_EQ_ADD_DIV) (SPEC (--`n:num`--) LESS_SUC_REFL)
+              ACARRY_EQ_ADD_DIV) (SPEC (--`n:num`--) LESS_SUC_REFL)
     in
     INDUCT_TAC THEN REPEAT RESQ_GEN_TAC THENL[
      ASSUM_LIST (fn asl =>  SUBST_TAC (map (MATCH_MP PWORDLEN0) asl))
@@ -583,37 +583,41 @@ val ACARRY_MSB = store_thm("ACARRY_MSB",
      THEN PURE_ONCE_REWRITE_TAC[ADD_ASSOC,EXP]
      THEN ASSUM_LIST (fn asl =>
         SUBST1_TAC (itlist (fn t1 => fn t2 => RESQ_MATCH_MP t2 t1)
-    	(butlast asl) (SPEC (--`n:num`--) ADD_BNVAL_LEFT)))
+        (butlast asl) (SPEC (--`n:num`--) ADD_BNVAL_LEFT)))
      THEN COND_REWRITE1_TAC
-    	 (GSYM (PURE_ONCE_REWRITE_RULE[MULT_SYM]DIV_DIV_DIV_MULT)) THENL[
+         (GSYM (PURE_ONCE_REWRITE_RULE[MULT_SYM]DIV_DIV_DIV_MULT)) THENL[
       MATCH_ACCEPT_TAC ZERO_LESS_TWO_EXP,
       MATCH_ACCEPT_TAC Less2,
       CONV_TAC ((RAND_CONV o ONCE_DEPTH_CONV) (REWR_CONV (GSYM ADD_ASSOC)))
       THEN COND_REWRITE1_TAC ADD_DIV_ADD_DIV
       THEN SUBST1_TAC lem1 THEN REWRITE_TAC[VB_MOD_2]
-      THEN CONV_TAC ((RAND_CONV o RAND_CONV o LHS_CONV o RAND_CONV)
-    	 (ONCE_DEPTH_CONV (REWR_CONV (GSYM ADD_ASSOC))))
+      THEN CONV_TAC ((RAND_CONV o RAND_CONV o LAND_CONV o RAND_CONV)
+         (ONCE_DEPTH_CONV (REWR_CONV (GSYM ADD_ASSOC))))
       THEN REFL_TAC]]
     end);
 
 (*-----------------------------------------------------------------------*)
-(* ACARRY_WSEG	    	    	    					*)
+(* ACARRY_WSEG                                                          *)
 (*-----------------------------------------------------------------------*)
 
 val ACARRY_WSEG = store_thm("ACARRY_WSEG",
     (--`!n. !w1 w2::PWORDLEN n. !cin k m. k < m /\ m <= n ==>
      (ACARRY k (WSEG m 0 w1) (WSEG m 0 w2) cin = ACARRY k w1 w2 cin)`--),
-    let val bit_seg = RESQ_GEN_ALL
-    	(REWRITE_RULE[LESS_MONO_EQ,LESS_EQ_MONO,ADD_CLAUSES]
-    	(GQSPECL[(--`SUC n`--), (--`w:bool word`--),
-                 (--`SUC m`--), (--`0`--), (--`k:num`--)] BIT_WSEG))
+    let val bit_seg =
+        CONV_RULE (HO_REWR_CONV (GSYM RES_FORALL))
+        (GEN ``w : bool word``
+         (DISCH_ALL
+          (REWRITE_RULE[LESS_MONO_EQ,LESS_EQ_MONO,ADD_CLAUSES]
+           (RESQ_SPECL[(--`SUC n`--), (--`w:bool word`--),
+                       (--`SUC m`--), (--`0`--), (--`k:num`--)]
+            (INST_TYPE [alpha |-> bool] BIT_WSEG)))))
     in
     INDUCT_TAC THEN REPEAT RESQ_GEN_TAC THEN GEN_TAC THENL[
       REPEAT GEN_TAC THEN DISCH_THEN (CONJUNCTS_THEN2 MP_TAC ASSUME_TAC)
       THEN IMP_RES_THEN SUBST1_TAC LESS_EQ_0_EQ
       THEN REWRITE_TAC[NOT_LESS_0],
       REPEAT INDUCT_TAC THEN REWRITE_TAC
-    	[NOT_LESS_0,LESS_MONO_EQ,LESS_EQ_MONO,ACARRY_DEF]
+        [NOT_LESS_0,LESS_MONO_EQ,LESS_EQ_MONO,ACARRY_DEF]
       THEN STRIP_TAC THEN IMP_RES_TAC LESS_SUC THEN AP_TERM_TAC
       THEN RESQ_REWRITE1_TAC bit_seg THEN AP_THM_TAC THEN AP_TERM_TAC
       THEN PURE_ONCE_REWRITE_TAC[ADD_ASSOC]
@@ -626,10 +630,10 @@ val ICARRY_WSEG = store_thm("ICARRY_WSEG",
     (--`!n. !w1 w2::PWORDLEN n. !cin k m. k < m /\ m <= n ==>
      (ICARRY k (WSEG m 0 w1) (WSEG m 0 w2) cin = ICARRY k w1 w2 cin)`--),
    let val i_eq_a = itlist DISCH [``k <= m``,
-                                  ``PWORDLEN m (WSEG m 0 w2:bool word)``,
-                                  ``PWORDLEN m (WSEG m 0 w1:bool word)``
+                                  ``(WSEG m 0 w2:bool word) IN PWORDLEN m``,
+                                  ``(WSEG m 0 w1:bool word) IN PWORDLEN m``
                                   ]
-     (SYM(UNDISCH_ALL(GQSPECL [(--`m:num`--),(--`WSEG m 0 (w1:bool word)`--),
+     (SYM(UNDISCH_ALL(RESQ_SPECL [(--`m:num`--),(--`WSEG m 0 (w1:bool word)`--),
      (--`WSEG m 0 (w2:bool word)`--), (--`cin:bool`--),(--`k:num`--)]  ACARRY_EQ_ICARRY)))
     in
     GEN_TAC THEN REPEAT RESQ_GEN_TAC THEN REPEAT GEN_TAC THEN STRIP_TAC
@@ -641,11 +645,11 @@ val ICARRY_WSEG = store_thm("ICARRY_WSEG",
       THEN ASM_REWRITE_TAC[ADD_0],
       RESQ_REWRITE1_TAC ACARRY_WSEG
       THEN RESQ_REWRITE1_TAC (SPEC (--`n:num`--) ACARRY_EQ_ICARRY) THENL[
-    	IMP_RES_TAC LESS_EQ_TRANS, REFL_TAC]]
+        IMP_RES_TAC LESS_EQ_TRANS, REFL_TAC]]
     end);
 
 (*-----------------------------------------------------------------------*)
-(* ACARRY_ACARRY_WSEG 	    	    					*)
+(* ACARRY_ACARRY_WSEG                                                   *)
 (*-----------------------------------------------------------------------*)
 
 val ACARRY_ACARRY_WSEG = store_thm("ACARRY_ACARRY_WSEG",
@@ -653,9 +657,13 @@ val ACARRY_ACARRY_WSEG = store_thm("ACARRY_ACARRY_WSEG",
      !cin m k1 k2. k1 < m /\ k2 < n /\ (m + k2) <= n ==>
      (ACARRY k1 (WSEG m k2 w1) (WSEG m k2 w2) (ACARRY k2 w1 w2 cin) =
        ACARRY (k1 + k2) w1 w2 cin)`--),
-    let val bit_seg = RESQ_GEN_ALL
-    	(GQSPECL[(--`SUC n`--),(--`w:bool word`--),(--`SUC m`--),
-                 (--`SUC k2`--),(--`k1:num`--)]BIT_WSEG)
+    let val bit_seg =
+          CONV_RULE (HO_REWR_CONV (GSYM RES_FORALL))
+          (GEN ``w : bool word``
+           (DISCH_ALL
+            (RESQ_SPECL[(--`SUC n`--),(--`w:bool word`--),(--`SUC m`--),
+                        (--`SUC k2`--),(--`k1:num`--)]
+             (INST_TYPE [alpha |-> bool] BIT_WSEG))))
     in
     INDUCT_TAC THEN REPEAT RESQ_GEN_TAC THEN GEN_TAC THENL[
      REWRITE_TAC[NOT_LESS_0],
@@ -666,9 +674,9 @@ val ACARRY_ACARRY_WSEG = store_thm("ACARRY_ACARRY_WSEG",
        INDUCT_TAC THENL[
         PURE_ONCE_REWRITE_TAC[ADD_0,(CONJUNCT1 ACARRY_DEF)]
         THEN STRIP_TAC THEN MATCH_MP_TAC
-    	 (GQSPECL [(--`SUC n`--), (--`w1:bool word`--),
-                   (--`w2:bool word`--), (--`cin:bool`--),
-    	    	  (--`SUC k1`--), (--`SUC m`--)] ACARRY_WSEG)
+         (RESQ_SPECL [(--`SUC n`--), (--`w1:bool word`--),
+                      (--`w2:bool word`--), (--`cin:bool`--),
+                      (--`SUC k1`--), (--`SUC m`--)] ACARRY_WSEG)
       THEN CONJ_TAC THEN FIRST_ASSUM ACCEPT_TAC,
       STRIP_TAC THEN PURE_ONCE_REWRITE_TAC[ADD]
       THEN PURE_ONCE_REWRITE_TAC[ACARRY_DEF] THEN AP_TERM_TAC
@@ -677,7 +685,7 @@ val ACARRY_ACARRY_WSEG = store_thm("ACARRY_ACARRY_WSEG",
       THEN PURE_ONCE_REWRITE_TAC[ADD_ASSOC]
       THEN PURE_ONCE_REWRITE_TAC[ADD_MONO_EQ] THEN AP_TERM_TAC
       THEN FIRST_ASSUM (IMP_RES_TAC o
-    	 (PURE_ONCE_REWRITE_RULE[LESS_EQ_MONO]) o (SPEC (--`SUC k2`--)))]]]]
+         (PURE_ONCE_REWRITE_RULE[LESS_EQ_MONO]) o (SPEC (--`SUC k2`--)))]]]]
     end);
 
 val _ = export_theory();
