src/word/theories/bword_numScript.sml
@@ -1,20 +1,22 @@
 (* ===================================================== *)
-(* FILE: mk_bword_num.ml	    DATE: 14 Aug 1992	*)
-(* AUTHOR: Wai WONG  	    	    			*)
-(* TRANSLATOR: Paul Curzon  2 June 1993, Sept 1994	*)
-(* Writes: bword_base.th	    	    		*)
-(* Uses: Libraries: more_lists res_quan			*)
-(* Description: Creates a theorey for mapping between 	*)
-(* natural numbers and boolean words	    	    	*)
+(* FILE: mk_bword_num.ml            DATE: 14 Aug 1992    *)
+(* AUTHOR: Wai WONG                                      *)
+(* TRANSLATOR: Paul Curzon  2 June 1993, Sept 1994       *)
+(* UPDATED for new res_quan theories by Joe Hurd, 2001   *)
+(* Writes: bword_base.th                                 *)
+(* Uses: Libraries: more_lists res_quan                  *)
+(* Description: Creates a theorey for mapping between    *)
+(* natural numbers and boolean words                     *)
 (* ===================================================== *)
 
 
 open HolKernel Parse boolLib Prim_rec numLib res_quanLib;
 open rich_listTheory pairTheory arithmeticTheory prim_recTheory numTheory;
-open Cond_rewrite Res_quan word_baseTheory word_bitopTheory word_numTheory;
+open Cond_rewrite word_baseTheory word_bitopTheory word_numTheory;
 open Base;
+open res_quanTheory bossLib pred_setTheory;
 
-infix THEN THENL THENC ORELSE ORELSEC;
+infix THEN THENL THENC ORELSE ORELSEC |->;
 
 val _ = new_theory "bword_num";
 
@@ -31,14 +33,14 @@ val word_INDUCT_TAC =
     end;
 
 val RESQ_WORDLEN_TAC =
-    (CONV_TAC RESQ_FORALL_CONV THEN word_INDUCT_TAC
-     THEN PURE_ONCE_REWRITE_TAC[word_baseTheory.PWORDLEN_DEF]
+    (CONV_TAC RES_FORALL_CONV THEN word_INDUCT_TAC
+     THEN PURE_ONCE_REWRITE_TAC[word_baseTheory.IN_PWORDLEN]
      THEN GEN_TAC THEN DISCH_TAC);
 
 
 
 (*---------------------------------------------------------------*)
-(* Mapping between (bool)word and num 				 *)
+(* Mapping between (bool)word and num                            *)
 (*---------------------------------------------------------------*)
 
 val BV_DEF = new_definition("BV_DEF",
@@ -76,11 +78,11 @@ val BNVAL_11_lem = prove((--`!m n p. m < p /\ n < p ==> ~((p + m) =  n)`--),
       REPEAT GEN_TAC THEN STRIP_TAC THEN PURE_ONCE_REWRITE_TAC[ADD_0]
       THEN CONV_TAC (RAND_CONV SYM_CONV) THEN IMP_RES_TAC LESS_NOT_EQ,
       INDUCT_TAC THEN GEN_TAC THEN STRIP_TAC THENL[
-    	PURE_ONCE_REWRITE_TAC[ADD_EQ_0]
-    	THEN PURE_ONCE_REWRITE_TAC[DE_MORGAN_THM]
-    	THEN DISJ2_TAC THEN MATCH_ACCEPT_TAC NOT_SUC,
-    	PURE_REWRITE_TAC[ADD_CLAUSES,INV_SUC_EQ]
-    	THEN IMP_RES_TAC SUC_LESS THEN RES_TAC]]);
+        PURE_ONCE_REWRITE_TAC[ADD_EQ_0]
+        THEN PURE_ONCE_REWRITE_TAC[DE_MORGAN_THM]
+        THEN DISJ2_TAC THEN MATCH_ACCEPT_TAC NOT_SUC,
+        PURE_REWRITE_TAC[ADD_CLAUSES,INV_SUC_EQ]
+        THEN IMP_RES_TAC SUC_LESS THEN RES_TAC]]);
 
 val BNVAL_11 = store_thm("BNVAL_11",
     (--`!w1 w2:(bool)word. (WORDLEN w1 = WORDLEN w2) ==>
@@ -98,12 +100,12 @@ val BNVAL_11 = store_thm("BNVAL_11",
       PURE_REWRITE_TAC[MULT_CLAUSES,ADD_CLAUSES]
       THEN ASSUME_TAC (ISPEC (--`l':bool list`--) lem2)
       THEN ASSUME_TAC(SUBS[ASSUME(--`LENGTH(l:bool list) = LENGTH(l':bool list)`--)]
-    	(ISPEC (--`l:bool list`--) lem2))
+        (ISPEC (--`l:bool list`--) lem2))
       THEN IMP_RES_TAC lem1 THEN ASM_REWRITE_TAC[],
       PURE_REWRITE_TAC[MULT_CLAUSES,ADD_CLAUSES]
       THEN ASSUME_TAC (ISPEC (--`l':bool list`--) lem2)
       THEN ASSUME_TAC(SUBS[ASSUME(--`LENGTH(l:bool list) = LENGTH(l':bool list)`--)]
-    	(ISPEC (--`l:bool list`--) lem2))
+        (ISPEC (--`l:bool list`--) lem2))
       THEN CONV_TAC ((RATOR_CONV o RAND_CONV) SYM_CONV)
       THEN IMP_RES_TAC lem1 THEN ASM_REWRITE_TAC[],
       PURE_REWRITE_TAC[MULT_CLAUSES,ADD_CLAUSES]
@@ -123,7 +125,7 @@ val BNVAL_MAX = store_thm("BNVAL_MAX",
     (--`!n. !w:(bool)word ::PWORDLEN n. BNVAL w < (2 EXP n)`--),
     GEN_TAC THEN RESQ_WORDLEN_TAC
     THEN PURE_REWRITE_TAC[BNVAL_DEF]
-    THEN FIRST_ASSUM SUBST1_TAC THEN MATCH_MP_TAC LVAL_MAX
+    THEN FIRST_ASSUM (SUBST1_TAC o SYM) THEN MATCH_MP_TAC LVAL_MAX
     THEN GEN_TAC THEN PURE_ONCE_REWRITE_TAC[BV_DEF]
     THEN COND_CASES_TAC THEN CONV_TAC (REDEPTH_CONV num_CONV)
     THEN REWRITE_TAC[LESS_0,LESS_MONO_EQ]);
@@ -136,21 +138,22 @@ val BNVAL_WCAT1 = store_thm("BNVAL_WCAT1",
     THEN PURE_ONCE_REWRITE_TAC[GSYM SNOC_APPEND]
     THEN MATCH_ACCEPT_TAC LVAL_SNOC);
 
-val BNVAL_WCAT2 = save_thm("BNVAL_WCAT2",
-   (* (--`!n. !w:(bool)word::PWORDLEN n.
+val BNVAL_WCAT2 = store_thm
+  ("BNVAL_WCAT2",
+   ``!n. !w:(bool)word::PWORDLEN n.
           !x:bool. BNVAL (WCAT (WORD[x],w))
-                   = ((BV x) 'a (2 EXP n)) + (BNVAL w)`--) *)
-    GEN_ALL (RESQ_GEN_ALL (GEN (--`x:bool`--)
-    (PURE_REWRITE_RULE[GSYM BNVAL_NVAL]
-        (ISPECL [(--`BV`--), (--`2`--), (--`x:bool`--)]
-                (RESQ_SPEC (--`w:bool word`--) (SPEC_ALL NVAL_WCAT2)))))));
+                   = ((BV x) * (2 EXP n)) + (BNVAL w)``,
+   REPEAT RESQ_STRIP_TAC
+   THEN MP_TAC ((RESQ_SPECL [``n : num``, ``w : bool word``, ``BV``, ``2``, ``x : bool``]) (INST_TYPE [alpha |-> bool] NVAL_WCAT2))
+   THEN PROVE_TAC [BNVAL_NVAL]);
 
-val BNVAL_WCAT = save_thm("BNVAL_WCAT",
-   GENL[(--`n:num`--),(--`m:num`--)]
-       (RESQ_GEN_ALL
-    (PURE_REWRITE_RULE[GSYM BNVAL_NVAL] (ISPECL [(--`BV`--), (--`2`--)]
-     (RESQ_SPECL [(--`w1:bool word`--),
-                  (--`w2:bool word`--)] (SPEC_ALL NVAL_WCAT))))));
+val BNVAL_WCAT = store_thm
+  ("BNVAL_WCAT",
+   ``!n m. !w1 :: PWORDLEN n. !w2 :: PWORDLEN m.
+       BNVAL (WCAT (w1, w2)) = (BNVAL w1 * (2 EXP m)) + (BNVAL w2)``,
+   REPEAT RESQ_STRIP_TAC
+   THEN MP_TAC ((RESQ_SPECL [``n : num``, ``m : num``, ``w1 : bool word``, ``w2 : bool word``, ``BV``, ``2``]) (INST_TYPE [alpha |-> bool] NVAL_WCAT))
+   THEN PROVE_TAC [BNVAL_NVAL]);
 
 val VB_DEF = new_definition("VB_DEF",
     (--`VB n = ~((n MOD 2) = 0)`--));
@@ -173,7 +176,7 @@ val WORDLEN_NBWORD = store_thm("WORDLEN_NBWORD",
     REWRITE_TAC[NBWORD_DEF,WORDLEN_DEF,NLIST_LENGTH]);
 
 val PWORDLEN_NBWORD = store_thm("PWORDLEN_NBWORD",
-    (--`!n m. PWORDLEN n (NBWORD n m)`--),
+    (--`!n m. (NBWORD n m) IN PWORDLEN n`--),
     REWRITE_TAC[PWORDLEN,WORDLEN_NBWORD]);
 
 val NBWORD_SUC = store_thm("NBWORD_SUC",
@@ -191,7 +194,7 @@ val VB_BV = store_thm("VB_BV", (--`!x. VB(BV x) = x`--),
 val BV_VB = store_thm("BV_VB", (--`!x. x < 2 ==> (BV(VB x) = x)`--),
     let val lem1 = SUBS[SYM (num_CONV (--`2`--))] (SPEC (--`1`--) LESS_0)
     val lems = map (fn th => MP(REWRITE_RULE[LESS_0] (SPEC (--`2`--) th)) lem1)
-    	[ZERO_DIV,ZERO_MOD]
+        [ZERO_DIV,ZERO_MOD]
    in
     CONV_TAC (REDEPTH_CONV num_CONV)
     THEN PURE_REWRITE_TAC[LESS_THM,NOT_LESS_0,OR_CLAUSES,BV_DEF,VB_DEF]
@@ -206,37 +209,37 @@ val NBWORD_BNVAL = store_thm("NBWORD_BNVAL",
     (--`!n. !w::PWORDLEN n. NBWORD n (BNVAL w) = w`--),
     GEN_TAC THEN RESQ_WORDLEN_TAC
     THEN PURE_REWRITE_TAC[BNVAL_DEF,NBWORD_DEF]
-    THEN FIRST_ASSUM SUBST1_TAC THEN PURE_ONCE_REWRITE_TAC[WORD_11]
+    THEN FIRST_ASSUM (SUBST1_TAC o SYM) THEN PURE_ONCE_REWRITE_TAC[WORD_11]
     THEN SPEC_TAC ((--`l: bool list`--),(--`l:bool list`--))
     THEN SNOC_INDUCT_TAC THEN REWRITE_TAC[LVAL_SNOC,LENGTH,LENGTH_SNOC,NLIST_DEF]
     THEN PURE_ONCE_REWRITE_TAC[MATCH_MP DIV_MULT (SPEC (--`h:bool`--) BV_LESS_2)]
     THEN GEN_TAC THEN PURE_ONCE_REWRITE_TAC[SNOC_11] THEN CONJ_TAC THENL[
       PURE_REWRITE_TAC[BV_DEF,VB_DEF]
       THEN COND_REWRITE1_TAC MOD_MOD THENL[
-    	CONV_TAC (RAND_CONV num_CONV) THEN MATCH_ACCEPT_TAC LESS_0,
+        CONV_TAC (RAND_CONV num_CONV) THEN MATCH_ACCEPT_TAC LESS_0,
         BOOL_CASES_TAC (--`x:bool`--) THENL[
           CONV_TAC (ONCE_DEPTH_CONV COND_CONV)
           THEN COND_REWRITE1_TAC MOD_TIMES
-    	  THEN COND_REWRITE1_TAC LESS_MOD THENL[
+          THEN COND_REWRITE1_TAC LESS_MOD THENL[
             CONV_TAC (TOP_DEPTH_CONV num_CONV)
-    	    THEN PURE_ONCE_REWRITE_TAC[LESS_MONO_EQ]
-    	    THEN MATCH_ACCEPT_TAC LESS_0,
-    	    REWRITE_TAC[SUC_ID]],
-    	  REWRITE_TAC[ADD_0] THEN MATCH_MP_TAC MOD_EQ_0
-    	  THEN FIRST_ASSUM ACCEPT_TAC]],
+            THEN PURE_ONCE_REWRITE_TAC[LESS_MONO_EQ]
+            THEN MATCH_ACCEPT_TAC LESS_0,
+            REWRITE_TAC[SUC_ID]],
+          REWRITE_TAC[ADD_0] THEN MATCH_MP_TAC MOD_EQ_0
+          THEN FIRST_ASSUM ACCEPT_TAC]],
       FIRST_ASSUM ACCEPT_TAC]);
 
 val BNVAL_NBWORD = store_thm("BNVAL_NBWORD",
     (--`!n m. (m < (2 EXP n)) ==> (BNVAL (NBWORD n m) = m)`--),
     let val SUM_LESS = ARITH_PROVE
-    	 (--`!m n p. ((m + n) < p) ==> ((m < p) /\ (n < p))`--)
+         (--`!m n p. ((m + n) < p) ==> ((m < p) /\ (n < p))`--)
     val lem1 = SUBS[SYM (num_CONV (--`2`--))] (SPEC (--`1`--) LESS_0)
     val lems = map (fn th => MP(REWRITE_RULE[LESS_0] (SPEC (--`2`--) th)) lem1)
-    	[ZERO_DIV,ZERO_MOD]
+        [ZERO_DIV,ZERO_MOD]
     val lem2 = RESQ_MATCH_MP (SPEC_ALL BNVAL_WCAT1)
      (SPECL [(--`n:num`--), (--`(SUC m) DIV 2`--)]PWORDLEN_NBWORD)
     val (lem31,lem32) =
-    	  CONJ_PAIR(SPEC (--`SUC m`--) (MP (SPEC (--`2`--) DIVISION) lem1))
+          CONJ_PAIR(SPEC (--`SUC m`--) (MP (SPEC (--`2`--) DIVISION) lem1))
     in
     REPEAT INDUCT_TAC THENL[
       REWRITE_TAC[NBWORD0,BNVAL_DEF,LVAL],
@@ -244,45 +247,43 @@ val BNVAL_NBWORD = store_thm("BNVAL_NBWORD",
       THEN REWRITE_TAC[LESS_MONO_EQ,NOT_LESS_0],
       DISCH_TAC THEN PURE_REWRITE_TAC[NBWORD_DEF,NLIST_DEF,BNVAL_DEF,LVAL_SNOC]
       THEN PURE_REWRITE_TAC lems THEN COND_REWRITE1_TAC BV_VB THENL[
-    	CONV_TAC (RAND_CONV num_CONV) THEN MATCH_ACCEPT_TAC LESS_0,
+        CONV_TAC (RAND_CONV num_CONV) THEN MATCH_ACCEPT_TAC LESS_0,
         FIRST_ASSUM (fn t => COND_REWRITE1_TAC (PURE_REWRITE_RULE
-    	  [NBWORD_DEF,BNVAL_DEF,LVAL_SNOC](SPEC (--`0`--) t))) THENL[
-    	  CONV_TAC (ONCE_DEPTH_CONV num_CONV)
-    	  THEN MATCH_ACCEPT_TAC ZERO_LESS_EXP,
-    	  REWRITE_TAC[MULT,ADD_0]]],
+          [NBWORD_DEF,BNVAL_DEF,LVAL_SNOC](SPEC (--`0`--) t))) THENL[
+          CONV_TAC (ONCE_DEPTH_CONV num_CONV)
+          THEN MATCH_ACCEPT_TAC ZERO_LESS_EXP,
+          REWRITE_TAC[MULT,ADD_0]]],
       DISCH_TAC THEN PURE_ONCE_REWRITE_TAC[NBWORD_SUC]
       THEN PURE_ONCE_REWRITE_TAC[lem2]
       THEN COND_REWRITE1_TAC BV_VB THENL[
-    	ACCEPT_TAC lem32,
-    	FIRST_ASSUM (fn t => COND_REWRITE1_TAC (SPEC (--`(SUC m) DIV 2`--) t)) THENL[
+        ACCEPT_TAC lem32,
+        FIRST_ASSUM (fn t => COND_REWRITE1_TAC (SPEC (--`(SUC m) DIV 2`--) t)) THENL[
           ACCEPT_TAC (PURE_ONCE_REWRITE_RULE[LESS_MULT_MONO]
-    	    (SUBS_OCCS[([1,3],(num_CONV (--`2`--)))]
-    	    (CONV_RULE ((RATOR_CONV o RAND_CONV) (REWR_CONV MULT_SYM))
-    	    (PURE_REWRITE_RULE[EXP] (CONJUNCT1 (MATCH_MP SUM_LESS
-    	    (SUBS [lem31](ASSUME (--`(SUC m) < (2 EXP (SUC n))`--))) )))))),
-    	  ACCEPT_TAC (SYM lem31)]]]
+            (SUBS_OCCS[([1,3],(num_CONV (--`2`--)))]
+            (CONV_RULE ((RATOR_CONV o RAND_CONV) (REWR_CONV MULT_SYM))
+            (PURE_REWRITE_RULE[EXP] (CONJUNCT1 (MATCH_MP SUM_LESS
+            (SUBS [lem31](ASSUME (--`(SUC m) < (2 EXP (SUC n))`--))) )))))),
+          ACCEPT_TAC (SYM lem31)]]]
      end);
 
-(* ZERO_WORD_VAL = |- !w :: PWORDLEN n. (w = NBWORD n 0) = (BNVAL w = 0) *)
-
-val ZERO_WORD_VAL = save_thm("ZERO_WORD_VAL",
-    GEN_ALL (RESQ_GEN_ALL
-    (RIGHT_CONV_RULE SYM_CONV (SYM (RIGHT_CONV_RULE SYM_CONV
-    (IMP_ANTISYM_RULE
-     (DISCH (--`0 = BNVAL w`--) (RIGHT_CONV_RULE
-       (RESQ_REWRITE1_CONV [] NBWORD_BNVAL)
-	 (AP_TERM (--`NBWORD n`--) (ASSUME (--`0 = BNVAL w`--)))))
-     (DISCH_ALL (SUBS[(MP (SPECL [(--`n:num`--),(--`0`--)] BNVAL_NBWORD)
-	 (SUBS[SYM(num_CONV (--`2`--))]
+val ZERO_WORD_VAL = store_thm
+  ("ZERO_WORD_VAL",
+   ``!w :: PWORDLEN n. (w = NBWORD n 0) = (BNVAL w = 0)``,
+   REPEAT (RESQ_STRIP_TAC ORELSE EQ_TAC) THENL
+   [PROVE_TAC [DISCH_ALL (SUBS[(MP (SPECL [(--`n:num`--),(--`0`--)] BNVAL_NBWORD)
+         (SUBS[SYM(num_CONV (--`2`--))]
           (SPECL [(--`n:num`--), (--`1`--)] ZERO_LESS_EXP)))]
-	  (AP_TERM (--`BNVAL`--) (ASSUME (--`NBWORD n 0 = w`--)))))) )))));
+          (AP_TERM (--`BNVAL`--) (ASSUME (--`NBWORD n 0 = w`--))))],
+    PROVE_TAC [(DISCH (--`0 = BNVAL w`--) (RIGHT_CONV_RULE
+       (RESQ_REWRITE1_CONV [] NBWORD_BNVAL)
+         (AP_TERM (--`NBWORD n`--) (ASSUME (--`0 = BNVAL w`--)))))]]);
 
 val WCAT_NBWORD_0 = store_thm("WCAT_NBWORD_0",
     (--`!n1 n2. WCAT((NBWORD n1 0), (NBWORD n2 0)) = (NBWORD (n1 + n2) 0)`--),
     let val lemma1 =
       let val lem1 = SUBS[SYM (num_CONV (--`2`--))] (SPEC (--`1`--) LESS_0)
       val lems = map (fn th => MP(REWRITE_RULE[LESS_0] (SPEC (--`2`--) th)) lem1)
-    	[ZERO_DIV,ZERO_MOD]
+        [ZERO_DIV,ZERO_MOD]
       in
         GEN_ALL(SUBS lems (SPECL [(--`n:num`--) , (--`0`--)] NBWORD_SUC))
       end
@@ -297,6 +298,7 @@ val WCAT_NBWORD_0 = store_thm("WCAT_NBWORD_0",
       THEN AP_TERM_TAC THEN ASM_REWRITE_TAC[PAIR_EQ]]
    end);
 
+(*|- !n m. m <= n ==> (WSPLIT m (NBWORD n 0) = (NBWORD (n - m) 0,NBWORD m 0))*)
 val WSPLIT_NBWORD_0 = save_thm("WSPLIT_NBWORD_0",
     let val tms = [(--`NBWORD (n-m) 0`--), (--`NBWORD m 0`--)]
     val ths = map (fn t => SPECL t PWORDLEN_NBWORD)
@@ -307,46 +309,51 @@ val WSPLIT_NBWORD_0 = save_thm("WSPLIT_NBWORD_0",
      (itlist PROVE_HYP ths
       (PURE_ONCE_REWRITE_RULE[WCAT_NBWORD_0]
        (RESQ_SPECL tms (SPECL [(--`n - m`--), (--`m:num`--)]
-        (CONJUNCT2(word_baseTheory.WORD_PARTITION))))))))
+        (INST_TYPE [alpha |-> bool]
+         (CONJUNCT2(word_baseTheory.WORD_PARTITION)))))))))
     end);
 
-val EQ_NBWORD0_SPLIT = store_thm("EQ_NBWORD0_SPLIT",
-    (--`!n. !w:(bool)word::PWORDLEN n. !m. m <= n ==>
-     ((w = NBWORD n 0) =
-      ((WSEG (n-m) m w = NBWORD (n-m) 0) /\
-       (WSEG m 0 w = NBWORD m 0)))`--),
-    let val lem0 = SPEC_ALL
-                (INST_TYPE [{residue =(==`:bool`==), redex =(==`:'a`==)}]
-    	(CONJUNCT1(word_baseTheory.WORD_PARTITION)))
-    val lem1 = SYM (UNDISCH_ALL (SPEC_ALL (RESQ_SPEC_ALL lem0)))
-    val lem4 = (SPECL[(--`n:num`--), (--`0`--)] PWORDLEN_NBWORD)
-    val lem3 = SYM (UNDISCH_ALL (SPEC_ALL (RESQ_MATCH_MP lem0 lem4)))
-    val lem2 = UNDISCH_ALL (SPEC (--`m:num`--) (RESQ_SPEC (--`w:bool word`--)
-    	    	 (SPEC_ALL (INST_TYPE [{residue =(==`:bool`==),
-                                        redex =(==`:'a`==)}] WSPLIT_WSEG))))
-    val lem5 = SPECL [(--`n-m`--), (--`m:num`--)] WCAT_11
-    val lem6 = (RESQ_SPEC (--`w:(bool)word`--)(SPEC (--`n:num`--) WSEG_PWORDLEN))
-    val lem7 = UNDISCH_ALL
-    	(PURE_ONCE_REWRITE_RULE[ADD_0] (SPECL[(--`m:num`--),(--`0`--)]lem6))
-    val lem8 =
-         let val lem = PURE_ONCE_REWRITE_RULE[ADD_SYM]
-    	    	(UNDISCH_ALL (SPECL[(--`n:num`--),(--`m:num`--)]SUB_ADD))
-         in
-    	    MP (SUBS[lem ]
-    	    (PURE_ONCE_REWRITE_RULE[ADD_SYM]
-              (SPECL [(--`n-m`--),(--`m:num`--)] lem6)))
-    	       (SPEC (--`n:num`--) LESS_EQ_REFL)
-         end
-    val [nbwm,nbwn] = map (fn tls => SPECL tls PWORDLEN_NBWORD)
-    	[[(--`m:num`--), (--`0`--)], [(--`n-m`--), (--`0`--)]]
-    val lem10 = itlist (fn t1 => fn t2 => RESQ_MATCH_MP t2 t1)
-    	[nbwm, lem7, nbwn, lem8] lem5
+val EQ_NBWORD0_SPLIT = store_thm
+  ("EQ_NBWORD0_SPLIT",
+   ``!n. !w :: PWORDLEN n. !m.
+       m <= n ==>
+       ((w = NBWORD n 0) =
+        ((WSEG (n-m) m w = NBWORD (n-m) 0) /\
+         (WSEG m 0 w = NBWORD m 0)))``,
+    let
+      val lem0 = SPEC_ALL
+        (INST_TYPE [{residue =(==`:bool`==), redex =(==`:'a`==)}]
+         (CONJUNCT1(word_baseTheory.WORD_PARTITION)))
+      val lem1 =
+        SYM (UNDISCH (RESQ_SPECL [``w : bool word``, ``m : num``] lem0))
+      val lem4 = (SPECL[(--`n:num`--), (--`0`--)] PWORDLEN_NBWORD)
+      val lem3 = SYM (UNDISCH_ALL (SPEC_ALL (RESQ_MATCH_MP lem0 lem4)))
+      val lem2 = UNDISCH_ALL (SPEC (--`m:num`--) (RESQ_SPEC (--`w:bool word`--)
+                                                  (SPEC_ALL (INST_TYPE [{residue =(==`:bool`==),
+                                                                         redex =(==`:'a`==)}] WSPLIT_WSEG))))
+      val lem5 = SPECL [(--`n-m`--), (--`m:num`--)] WCAT_11
+      val lem6 = (RESQ_SPEC (--`w:(bool)word`--)(SPEC (--`n:num`--) (INST_TYPE [alpha |-> bool] WSEG_PWORDLEN)))
+      val lem7 = UNDISCH_ALL
+        (PURE_ONCE_REWRITE_RULE[ADD_0] (SPECL[(--`m:num`--),(--`0`--)]lem6))
+      val lem8 =
+        let val lem = PURE_ONCE_REWRITE_RULE[ADD_SYM]
+          (UNDISCH_ALL (SPECL[(--`n:num`--),(--`m:num`--)]SUB_ADD))
+        in
+          MP (SUBS[lem ]
+              (PURE_ONCE_REWRITE_RULE[ADD_SYM]
+               (SPECL [(--`n-m`--),(--`m:num`--)] lem6)))
+          (SPEC (--`n:num`--) LESS_EQ_REFL)
+        end
+      val [nbwm,nbwn] = map (fn tls => SPECL tls PWORDLEN_NBWORD)
+        [[(--`m:num`--), (--`0`--)], [(--`n-m`--), (--`0`--)]]
+      val lem10 = itlist (fn t1 => fn t2 => RESQ_MATCH_MP t2 t1)
+        [nbwm, lem7, nbwn, lem8] lem5
     in
-    GEN_TAC THEN RESQ_HALF_GEN_TAC THEN GEN_TAC THEN REPEAT STRIP_TAC
-    THEN SUBST_OCCS_TAC[([1],lem1), ([1],lem3)]
-    THEN ASSUME_TAC lem4 THEN SUBST1_TAC lem2
-    THEN COND_REWRITE1_TAC WSPLIT_NBWORD_0
-    THEN ACCEPT_TAC lem10
+      GEN_TAC THEN CONV_TAC RES_FORALL_CONV THEN GEN_TAC THEN REPEAT STRIP_TAC
+      THEN SUBST_OCCS_TAC[([1],lem1), ([1],lem3)]
+      THEN ASSUME_TAC lem4 THEN SUBST1_TAC lem2
+      THEN COND_REWRITE1_TAC WSPLIT_NBWORD_0
+      THEN ACCEPT_TAC lem10
     end);
 
 val LESS2_DIV2 = prove(
@@ -354,8 +361,8 @@ val LESS2_DIV2 = prove(
     REPEAT INDUCT_TAC THENL[
       REWRITE_TAC[NOT_LESS_0],
       STRIP_TAC THEN COND_REWRITE1_TAC ZERO_DIV THENL[
-    	CONV_TAC (RAND_CONV num_CONV) THEN MATCH_ACCEPT_TAC LESS_0,
-    	FIRST_ASSUM ACCEPT_TAC],
+        CONV_TAC (RAND_CONV num_CONV) THEN MATCH_ACCEPT_TAC LESS_0,
+        FIRST_ASSUM ACCEPT_TAC],
       REWRITE_TAC[NOT_LESS_0],
     PURE_ONCE_REWRITE_TAC[MULT_CLAUSES]
     THEN SUBST_OCCS_TAC[([1],(num_CONV(--`2`--)))] THEN SUBST1_TAC(num_CONV(--`1`--))
@@ -373,10 +380,10 @@ val LESS2_DIV2 = prove(
       THEN PURE_ONCE_REWRITE_TAC[ADD1] THEN PURE_ONCE_REWRITE_TAC[MULT_SYM]
       THEN COND_REWRITE1_TAC ADD_DIV_ADD_DIV THENL[
          CONV_TAC (REDEPTH_CONV num_CONV) THEN REWRITE_TAC[LESS_0],
-    	 COND_REWRITE1_TAC LESS_DIV_EQ_ZERO THENL[
+         COND_REWRITE1_TAC LESS_DIV_EQ_ZERO THENL[
            CONV_TAC (REDEPTH_CONV num_CONV)
-    	   THEN REWRITE_TAC[LESS_0,LESS_MONO_EQ],
-    	   MATCH_ACCEPT_TAC ADD_0]],
+           THEN REWRITE_TAC[LESS_0,LESS_MONO_EQ],
+           MATCH_ACCEPT_TAC ADD_0]],
       POP_ASSUM SUBST1_TAC THEN DISJ1_TAC THEN PURE_ONCE_REWRITE_TAC[MULT_SYM]
       THEN MATCH_MP_TAC MULT_DIV THEN CONV_TAC (REDEPTH_CONV num_CONV)
       THEN REWRITE_TAC[LESS_0],
@@ -415,22 +422,22 @@ val NBWORD_MOD = store_thm("NBWORD_MOD",
    (NBWORD n((m MOD (2 EXP (SUC n))) DIV 2) = NBWORD n(m DIV 2)) /\
    (WORD[VB((m MOD (2 EXP (SUC n))) MOD 2)] = WORD[VB(m MOD 2)]) *)
         let val tms1 = [(--`NBWORD n((m MOD (2 EXP (SUC n))) DIV 2)`--),
-    	    (--`NBWORD n(m DIV 2)`--)]
+            (--`NBWORD n(m DIV 2)`--)]
         val tms2 = [(--`WORD[VB((m MOD (2 EXP (SUC n))) MOD 2)]`--),
-    	    (--`WORD[VB(m MOD 2)]`--)]
+            (--`WORD[VB(m MOD 2)]`--)]
         val lem1 = RESQ_SPECL (tms1 @ tms2)
-                        (SPECL[(--`n:num`--),(--`1`--)] WCAT_11)
-    	val lems2 =
-    	    let val lm =  GEN_ALL (REWRITE_RULE[LENGTH]
-        	(RIGHT_CONV_RULE ((RATOR_CONV o RAND_CONV) num_CONV)
-    		 (SPECL [(--`1`--), (--`[x:'a]`--)] PWORDLEN_DEF)))
+                        (SPECL[(--`n:num`--),(--`1`--)] (INST_TYPE [alpha |-> bool] WCAT_11))
+        val lems2 =
+            let val lm =  GEN_ALL (REWRITE_RULE[LENGTH]
+                (RIGHT_CONV_RULE (RAND_CONV num_CONV)
+                 (SPECL [(--`1`--), (--`[x:'a]`--)] IN_PWORDLEN)))
             in
-    	       map (fn t =>
+               map (fn t =>
                     ISPEC (hd (#1 (listSyntax.dest_list
                                    (#Rand(dest_comb t))))) lm) tms2
             end
         val lems3 =
-    	    map (fn t => ISPECL (snd (strip_comb t)) PWORDLEN_NBWORD) tms1
+            map (fn t => ISPECL (snd (strip_comb t)) PWORDLEN_NBWORD) tms1
         in
          (itlist PROVE_HYP (lems2 @ lems3) lem1)
         end
@@ -440,15 +447,15 @@ val NBWORD_MOD = store_thm("NBWORD_MOD",
       REWRITE_TAC[NBWORD_SUC] THEN GEN_TAC
       THEN SUBST1_TAC lemma1 THEN CONJ_TAC THEN PURE_ONCE_REWRITE_TAC[EXP]
       THENL[
-    	COND_REWRITE1_TAC MOD_DIV_lemma THENL[
-    	  CONV_TAC (ONCE_DEPTH_CONV num_CONV)
-    	  THEN MATCH_ACCEPT_TAC ZERO_LESS_EXP,
-    	  FIRST_ASSUM MATCH_ACCEPT_TAC],
-    	COND_REWRITE1_TAC MOD_MULT_MOD THENL[
-    	  CONV_TAC (ONCE_DEPTH_CONV num_CONV) THEN MATCH_ACCEPT_TAC LESS_0,
-    	  CONV_TAC (ONCE_DEPTH_CONV num_CONV)
-    	  THEN MATCH_ACCEPT_TAC ZERO_LESS_EXP,
-    	  REFL_TAC]]]
+        COND_REWRITE1_TAC MOD_DIV_lemma THENL[
+          CONV_TAC (ONCE_DEPTH_CONV num_CONV)
+          THEN MATCH_ACCEPT_TAC ZERO_LESS_EXP,
+          FIRST_ASSUM MATCH_ACCEPT_TAC],
+        COND_REWRITE1_TAC MOD_MULT_MOD THENL[
+          CONV_TAC (ONCE_DEPTH_CONV num_CONV) THEN MATCH_ACCEPT_TAC LESS_0,
+          CONV_TAC (ONCE_DEPTH_CONV num_CONV)
+          THEN MATCH_ACCEPT_TAC ZERO_LESS_EXP,
+          REFL_TAC]]]
     end);
 
 val WSEG_NBWORD_SUC = store_thm("WSEG_NBWORD_SUC",
@@ -479,23 +486,23 @@ val NBWORD_SUC_WSEG = store_thm("NBWORD_SUC_WSEG",
     THEN FIRST_ASSUM (fn t => SUBST_OCCS_TAC [([1],(RESQ_MATCH_MP
         (SPEC_ALL WORDLEN_SUC_WCAT_BIT_WSEG) t))])
     THEN PURE_ONCE_REWRITE_TAC[BNVAL_NVAL]
-    THEN `PWORDLEN n (WSEG n 0 w)` by
+    THEN `(WSEG n 0 w) IN PWORDLEN n` by
        (RESQ_IMP_RES_TAC WSEG_PWORDLEN THEN
         simpLib.ASM_SIMP_TAC bossLib.arith_ss [])
     THEN FIRST_ASSUM (fn t => PURE_ONCE_REWRITE_TAC
-    	[(RESQ_MATCH_MP (SPEC_ALL NVAL_WCAT2) t)])
+        [(RESQ_MATCH_MP (SPEC_ALL NVAL_WCAT2) t)])
     THEN PURE_ONCE_REWRITE_TAC[GSYM NBWORD_MOD]
     THEN COND_REWRITE1_TAC MOD_MULT THENL[
-    	RESQ_IMP_RES_TAC (MATCH_MP NVAL_MAX BV_LESS_2),
-    	PURE_ONCE_REWRITE_TAC[GSYM BNVAL_NVAL]
-    	THEN RESQ_IMP_RES_TAC NBWORD_BNVAL]);
+        RESQ_IMP_RES_TAC (MATCH_MP NVAL_MAX BV_LESS_2),
+        PURE_ONCE_REWRITE_TAC[GSYM BNVAL_NVAL]
+        THEN RESQ_IMP_RES_TAC NBWORD_BNVAL]);
 
 val DOUBLE_EQ_SHL = store_thm("DOUBL_EQ_SHL",
     (--`!n. 0 < n ==>  !w::PWORDLEN n. !b.
      (NBWORD n ((BNVAL w) + (BNVAL w) + (BV b))) = SND(SHL F w b)`--),
     let val WORD1 = REWRITE_RULE[LENGTH]
                         (RIGHT_CONV_RULE(ONCE_DEPTH_CONV num_CONV)
-    	(ISPECL [(--`1`--), (--`[b:bool]`--)] PWORDLEN_DEF))
+        (ISPECL [(--`1`--), (--`[b:bool]`--)] IN_PWORDLEN))
     val bnval_lem = (SPECL[(--`n:num`--),(--`BNVAL w`--)]PWORDLEN_NBWORD)
     in
     PURE_ONCE_REWRITE_TAC[ADD_ASSOC,SHL_DEF]
@@ -510,13 +517,13 @@ val DOUBLE_EQ_SHL = store_thm("DOUBL_EQ_SHL",
     THEN PURE_ONCE_REWRITE_TAC[PRE] THEN GEN_TAC
     THEN RESQ_IMP_RES_THEN
              (fn t => ASSUME_TAC(REWRITE_RULE[ADD,LESS_EQ_SUC_REFL]
-    	(SPECL[(--`n:num`--),(--`0`--)] t))) WSEG_PWORDLEN
+        (SPECL[(--`n:num`--),(--`0`--)] t))) WSEG_PWORDLEN
     THEN AP_TERM_TAC THEN REWRITE_TAC[PAIR_EQ]
     THEN RESQ_IMP_RES_TAC NBWORD_SUC_WSEG
    end);
 
 val ZERO_LESS_TWO_EXP = (GEN_ALL(SUBS[SYM(num_CONV (--`2`--))]
-    	(SPECL[(--`m:num`--),(--`1`--)]ZERO_LESS_EXP)));
+        (SPECL[(--`m:num`--),(--`1`--)]ZERO_LESS_EXP)));
 
 val MSB_NBWORD = store_thm("MSB_NBWORD",
     (--`!n m. BIT n (NBWORD (SUC n) m) = VB((m DIV (2 EXP n)) MOD 2)`--),
@@ -541,8 +548,8 @@ val NBWORD_SPLIT = store_thm("NBWORD_SPLIT",
     (--`!n1 n2 m. NBWORD (n1 + n2) m =
      WCAT ((NBWORD n1 (m DIV (2 EXP n2))), (NBWORD n2 m))`--),
     let val  exp_lems =
-    	let val lm = CONJUNCT2 EXP in
-    	(map GSYM [lm, PURE_ONCE_REWRITE_RULE[MULT_SYM]lm])
+        let val lm = CONJUNCT2 EXP in
+        (map GSYM [lm, PURE_ONCE_REWRITE_RULE[MULT_SYM]lm])
         end
     in
     INDUCT_TAC THENL[
@@ -566,9 +573,9 @@ val WSEG_NBWORD = store_thm("WSEG_NBWORD",
     (--`!m k n.  (m + k) <= n ==>
      (!l. WSEG m k(NBWORD n l) = NBWORD m (l DIV (2 EXP k)))`--),
     let val lem1 = CONV_RULE (COND_REWRITE1_CONV [] SUB_ADD)
-    	(SPECL[(--`n-k`--), (--`k:num`--), (--`l:num`--)]NBWORD_SPLIT)
+        (SPECL[(--`n-k`--), (--`k:num`--), (--`l:num`--)]NBWORD_SPLIT)
     val lem2 = CONV_RULE (COND_REWRITE1_CONV [] SUB_ADD)
-    	(SPECL[(--`(n-k)-m`--), (--`m:num`--)]NBWORD_SPLIT)
+        (SPECL[(--`(n-k)-m`--), (--`m:num`--)]NBWORD_SPLIT)
     in
     REPEAT STRIP_TAC THEN IMP_RES_TAC LESS_EQ_SPLIT
     THEN SUBST1_TAC lem1
@@ -598,8 +605,8 @@ val BIT_NBWORD0 = store_thm("BIT_NBWORD0",
     let val les1 = SUBS[SYM (num_CONV (--`1`--))](SPEC(--`0`--)LESS_SUC_REFL)
        val lem1 = REWRITE_RULE[ADD,les1]
                 (PROVE_HYP (SPECL [(--`n:num`--),(--`0`--)]PWORDLEN_NBWORD)
-     (GQSPECL[(--`n:num`--),(--`NBWORD n 0`--),(--`1`--),
-               (--`k:num`--),(--`0`--)]BIT_WSEG))
+     (RESQ_SPECL[(--`n:num`--),(--`NBWORD n 0`--),(--`1`--),
+               (--`k:num`--),(--`0`--)](INST_TYPE [alpha |-> bool]BIT_WSEG)))
     in
     REPEAT STRIP_TAC THEN COND_REWRITE1_TAC (GSYM lem1) THENL[
      ARITH_TAC,
@@ -614,7 +621,7 @@ val BIT_NBWORD0 = store_thm("BIT_NBWORD0",
 
 val add_lem = prove(
     (--`!m1 m2 n1 n2 p. (((m1 * p) + n1)  + ((m2 * p) + n2) =
-    	((m1 * p) + (m2 * p)) + (n1 + n2))`--),
+        ((m1 * p) + (m2 * p)) + (n1 + n2))`--),
     REPEAT GEN_TAC THEN PURE_ONCE_REWRITE_TAC[GSYM ADD_ASSOC]
     THEN PURE_ONCE_REWRITE_TAC[ADD_SYM]
     THEN PURE_ONCE_REWRITE_TAC[EQ_MONO_ADD_EQ]
@@ -626,18 +633,18 @@ val ADD_BNVAL_LEFT = store_thm("ADD_BNVAL_LEFT",
       (((BV (BIT n w1)) + (BV (BIT n w2))) * (2 EXP n)) +
        ((BNVAL (WSEG n 0 w1)) + (BNVAL (WSEG n 0 w2)))`--),
     let val mk_lem =
-    	let val lem = SPEC_ALL WSEG_PWORDLEN
-    	val lem2 = SPEC_ALL BNVAL_WCAT2
+        let val lem = SPEC_ALL WSEG_PWORDLEN
+        val lem2 = SPEC_ALL BNVAL_WCAT2
         in
-    	(fn t => RESQ_MATCH_MP lem2
-    	    (REWRITE_RULE[ADD_0,LESS_EQ_SUC_REFL]
+        (fn t => RESQ_MATCH_MP lem2
+            (REWRITE_RULE[ADD_0,LESS_EQ_SUC_REFL]
                      (SPECL[(--`n:num`--), (--`0`--)]
-    	    (RESQ_MATCH_MP lem t))))
+            (RESQ_MATCH_MP lem t))))
         end
    in
     GEN_TAC THEN REPEAT RESQ_GEN_TAC
     THEN EVERY_ASSUM (fn t =>SUBST_OCCS_TAC [([1],
-    		(RESQ_MATCH_MP (SPEC_ALL WORDLEN_SUC_WCAT_BIT_WSEG) t))])
+                (RESQ_MATCH_MP (SPEC_ALL WORDLEN_SUC_WCAT_BIT_WSEG) t))])
     THEN EVERY_ASSUM ((fn t => REWRITE_TAC[t]) o mk_lem)
     THEN PURE_ONCE_REWRITE_TAC[add_lem]
     THEN REWRITE_TAC[RIGHT_ADD_DISTRIB]
@@ -649,18 +656,18 @@ val ADD_BNVAL_RIGHT = store_thm("ADD_BNVAL_RIGHT",
       (((BNVAL (WSEG n 1 w1)) + (BNVAL (WSEG n 1 w2))) * 2) +
        ((BV (BIT 0 w1)) + (BV (BIT 0 w2))) `--),
     let val mk_lem =
-    	let val lem = SPEC_ALL WSEG_PWORDLEN
-    	val lem2 = SPEC_ALL BNVAL_WCAT1
+        let val lem = SPEC_ALL WSEG_PWORDLEN
+        val lem2 = SPEC_ALL BNVAL_WCAT1
         in
-    	(fn t => RESQ_MATCH_MP lem2
-    	    (REWRITE_RULE[GSYM ADD1,LESS_EQ_REFL]
+        (fn t => RESQ_MATCH_MP lem2
+            (REWRITE_RULE[GSYM ADD1,LESS_EQ_REFL]
             (SPECL[(--`n:num`--), (--`1`--)]
-    	    (RESQ_MATCH_MP lem t))))
+            (RESQ_MATCH_MP lem t))))
        end
     in
     GEN_TAC THEN REPEAT RESQ_GEN_TAC
     THEN EVERY_ASSUM (fn t => SUBST_OCCS_TAC [([1],
-	(RESQ_MATCH_MP (SPEC_ALL WORDLEN_SUC_WCAT_BIT_WSEG_RIGHT) t))])
+        (RESQ_MATCH_MP (SPEC_ALL WORDLEN_SUC_WCAT_BIT_WSEG_RIGHT) t))])
     THEN EVERY_ASSUM ((fn t =>REWRITE_TAC[t]) o mk_lem)
     THEN PURE_ONCE_REWRITE_TAC[add_lem]
     THEN REWRITE_TAC[RIGHT_ADD_DISTRIB]
@@ -671,11 +678,15 @@ val ADD_BNVAL_SPLIT = store_thm("ADD_BNVAL_SPLIT",
      ((BNVAL w1) + (BNVAL w2)) =
       (((BNVAL (WSEG n1 n2 w1)) + (BNVAL (WSEG n1 n2 w2))) * (2 EXP n2)) +
        ((BNVAL (WSEG n2 0 w1)) + (BNVAL (WSEG n2 0 w2)))`--),
-    let val seg_lem = PURE_ONCE_REWRITE_RULE[ADD_SYM](RESQ_GEN_ALL (SYM (TRANS
-    	(REWRITE_RULE[LESS_EQ_REFL] (PURE_ONCE_REWRITE_RULE[ADD_0]
-               (SPECL [(--`n2:num`--), (--`n1:num`--), (--`0`--)]
-    	 (RESQ_SPEC_ALL (SPEC (--`n2 + n1`--) WCAT_WSEG_WSEG)))))
-        (RESQ_SPEC_ALL (SPEC (--`n2 + n1`--) WSEG_WORD_LENGTH)))))
+    let val seg_lem = PURE_ONCE_REWRITE_RULE[ADD_SYM]
+        (CONV_RULE (HO_REWR_CONV (GSYM RES_FORALL))
+        (GEN ``w : 'a word``
+        (DISCH_ALL
+         (SYM
+          (TRANS
+           (REWRITE_RULE[LESS_EQ_REFL] (PURE_ONCE_REWRITE_RULE[ADD_0]
+               (RESQ_SPECL [``n2 + n1``, ``w : 'a word``, ``n2:num``, ``n1:num``, ``0``] WCAT_WSEG_WSEG)))
+           (RESQ_SPECL [``n2 + n1``, ``w : 'a word``] WSEG_WORD_LENGTH))))))
     val lem = SPEC_ALL WSEG_PWORDLEN
     val lem2 = SPECL [(--`n1:num`--), (--`n2:num`--)] BNVAL_WCAT
     val LESS_EQ_ADD2 = PURE_ONCE_REWRITE_RULE[ADD_SYM]LESS_EQ_ADD
@@ -685,8 +696,8 @@ val ADD_BNVAL_SPLIT = store_thm("ADD_BNVAL_SPLIT",
            (fn t => SUBST_OCCS_TAC [([1], (RESQ_MATCH_MP seg_lem t))])
     THEN RESQ_REWRITE1_TAC lem2
     THEN TRY
-    	(RULE_ASSUM_TAC (RESQ_MATCH_MP lem) THEN FIRST_ASSUM MATCH_MP_TAC
-    	 THEN REWRITE_TAC[ADD_0,LESS_EQ_ADD2,LESS_EQ_REFL])
+        (RULE_ASSUM_TAC (RESQ_MATCH_MP lem) THEN FIRST_ASSUM MATCH_MP_TAC
+         THEN REWRITE_TAC[ADD_0,LESS_EQ_ADD2,LESS_EQ_REFL])
     THEN PURE_ONCE_REWRITE_TAC[add_lem]
     THEN REWRITE_TAC[RIGHT_ADD_DISTRIB]
    end);
